Added spec to the library

alpha_map.fst
@@ -3,13 +3,32 @@ open FStar.List.Tot
 
 open Library
 
-type op (alpha_op:eqtype) = (nat (*key*) * alpha_op)
+type op (alpha_op:eqtype) = 
+  |Get : nat (*key*) -> alpha_op -> op (alpha_op)
+  |Set : nat (*key*) -> alpha_op -> op (alpha_op)
 
-val get_key : #o:eqtype -> op1:(nat * op o) -> Tot (k:nat {exists id op2. op1 = (id, (k, op2))})
-let get_key (id, (k, _)) = k
+val get_key : #o:eqtype -> op1:(nat * op o) -> Tot (k:nat {(exists id op2. op1 = (id, (Get k op2))) \/ 
+                                                     (exists id op2. op1 = (id, (Set k op2)))})
+let get_key op1 =
+  match op1 with
+  |(_, Get k _) -> k
+  |(_, Set k _) -> k
 
-val get_val : #o:eqtype -> op1:(nat * op o) -> Tot (s:o {exists id k. op1 = (id, (k, s))})
-let get_val (id, (k, s)) = s
+  val opget : #o:eqtype -> o1:(nat * (op o)) -> Tot (b:bool {b=true <==> (exists id k alphaop. (o1 = (id, (Get k alphaop))))})
+  let opget op1 =
+    match op1 with
+    |(_, (Get _ _)) -> true
+    |_ -> false
+
+  val opset : #o:eqtype -> o1:(nat * (op o)) -> Tot (b:bool {b=true <==> (exists id k alphaop. (o1 = (id, (Set k alphaop))))})
+  let opset op1 = not (opget op1)
+  
+val get_alpha_op : #o:eqtype -> op1:(nat * op o) -> Tot (s:o {(exists id k. op1 = (id, (Get k s))) \/
+                                                          (exists id k. op1 = (id, (Set k s)))})
+let get_alpha_op op1 =
+  match op1 with
+  |(_, Get _ o) -> o
+  |(_, Set _ o) -> o
 
 val get_key_s : #st:eqtype -> s:(nat * st) -> Tot (s1:nat {(exists c. s = (s1,c))})
 let get_key_s (k, _) = k
@@ -36,14 +55,14 @@ type s (alpha_st:eqtype) = l:list (nat * alpha_st) {unique_key l}
 
 let init_a = []
 
-val get_val_s : #st:eqtype -> #o:eqtype -> {| mrdt st o |}
+val get_val_s : #st:eqtype -> #o:eqtype -> #r:eqtype -> {| mrdt st o r|}
                 -> i:nat -> s1:s st -> Tot (c:st {(mem_key_s i s1 ==> mem (i,c) s1 /\ 
                                          (exists e. mem e s1 /\ e = (i,c) /\ c = get_val_s1 #st e)) /\ 
-                                         (not (mem_key_s i s1) ==> c = init #st #o)})
-let rec get_val_s #st #o i s1 =
+                                         (not (mem_key_s i s1) ==> c = init #st #o #r)})
+let rec get_val_s #st #o #r i s1 =
   match s1 with
-  |[] -> init #st #o
-  |x::xs -> if get_key_s x = i then get_val_s1 x else get_val_s #st #o i xs
+  |[] -> init #st #o #r
+  |x::xs -> if get_key_s x = i then get_val_s1 x else get_val_s #st #o #r i xs
 
 val mem_op : #o:eqtype -> ele1:op o
            -> l:list (nat * (op o))
@@ -53,11 +72,13 @@ let rec mem_op ele2 l =
   |[] -> false
   |(_, ele1)::xs -> ele1 = ele2 || mem_op ele2 xs
 
-val mem_key : #o:eqtype -> i:nat -> l:list (nat * op o) -> Tot (b:bool {b=true <==> (exists id op. mem (id, (i, op)) l)})
+val mem_key : #o:eqtype -> i:nat -> l:list (nat * op o) -> Tot (b:bool {b=true <==> (exists id op. mem (id, (Get i op)) l) \/
+                                                                           (exists id op. mem (id, (Set i op)) l)})
 let rec mem_key ele2 l =
   match l with
   |[] -> false
-  |(_, (ele1, _))::xs -> ele1 = ele2 || mem_key ele2 xs
+  |(_, (Get ele1 _))::xs -> ele1 = ele2 || mem_key ele2 xs
+  |(_, (Set ele1 _))::xs -> ele1 = ele2 || mem_key ele2 xs
 
 val filter_uni : #op:eqtype 
                -> f:((nat * op) -> bool)
@@ -72,63 +93,91 @@ let rec filter_uni f l =
 
 val project_op : #o:eqtype 
                -> o1:(nat * (op o))
-               -> Tot (o2:(nat * o) {o2 = (get_id o1, get_val o1)})
+               -> Tot (o2:(nat * o) {(o2 = (get_id o1, get_alpha_op o1))})
 let project_op op =
   match op with
-  |(id, (k, value)) -> (id, value)
+  |(id, (Set k alpha_op)) -> (id, alpha_op)
+  |(id, (Get k alpha_op)) -> (id, alpha_op)
 
 val project1 : #o:eqtype
              -> i:nat
              -> l:ae (op o)
              -> Pure (list (nat * o))
                     (requires true)
-                    (ensures (fun r -> (forall id. mem_id id r <==> (mem_id id l.l /\ get_key (get_eve id l.l) = i)) /\ 
-                                         unique_id r /\ (forall e. mem e l.l /\ get_key e = i ==> mem (project_op e) r)))
+                    (ensures (fun r -> (forall id. mem_id id r <==> (mem_id id l.l /\ get_key (get_eve id l.l) = i /\ 
+                      opset (get_eve id l.l))) /\ unique_id r /\ (forall e ao. mem e l.l /\ get_op e = (Set i ao) ==> (exists e1. mem e1 r /\ e1 = (get_id e, ao))) /\ (forall e. mem e l.l /\ get_key e = i /\ opset e ==> mem (project_op e) r)))
                (decreases List.Tot.length l.l)
 
 #set-options "--z3rlimit 10000000"
-let rec project1 i l =
+let rec project1 #o i l =
   match l.l with
   |[] -> []
-  |x::xs -> if (get_key x = i) then (project_op x)::project1 i (A l.vis xs) else (project1 i (A l.vis xs))
+  |x::xs -> if (get_key x = i && opset x) then (project_op x)::project1 i (A l.vis xs) else (project1 i (A l.vis xs))
+  (*)|(id, (Set k oper))::xs -> if i = id then (id, oper)::project1 #o i (A l.vis xs) else project1 #o i (A l.vis xs)
+  |(id, (Get _ _))::xs -> project1 #o i (A l.vis xs)*)
 
 val project : #o:eqtype
             -> i:nat
             -> l:ae (op o)
             -> Pure (ae o)
                    (requires true)
-                   (ensures (fun r -> (forall id. mem_id id r.l <==> (mem_id id l.l /\ get_key (get_eve id l.l) = i)) /\ 
-                                     unique_id r.l /\ (forall e. mem e l.l /\ get_key e = i ==> mem (project_op e) r.l) /\
-                   (forall e e1. (get_id e <> get_id e1 /\ mem (get_id e, (i, get_op e)) l.l /\ 
-             mem (get_id e1, (i, get_op e1)) l.l /\ l.vis (get_id e, (i, get_op e)) (get_id e1, (i, get_op e1))) <==> 
-                   (get_id e <> get_id e1 /\ mem e r.l /\ mem e1 r.l /\ r.vis e e1)) /\ not (mem_key i l.l) <==> r.l = []))
+                   (ensures (fun r -> (forall id. mem_id id r.l <==> (mem_id id l.l /\ opset (get_eve id l.l) /\ get_key (get_eve id l.l) = i)) /\ 
+                       unique_id r.l /\ (forall e ao. mem e l.l /\ get_op e = (Set i ao) ==> (exists e1. mem e1 r.l /\ e1 = (get_id e, ao))) /\ (forall e. mem e l.l /\ get_key e = i /\ opset e ==> mem (project_op e) r.l) /\
+                   (forall e e1. (get_id e <> get_id e1 /\ mem (get_id e, (Set i (get_op e))) l.l /\ 
+             mem (get_id e1, (Set i (get_op e1))) l.l /\ l.vis (get_id e, (Set i (get_op e))) (get_id e1, (Set i (get_op e1)))) <==> 
+                   (get_id e <> get_id e1 /\ mem e r.l /\ mem e1 r.l /\ r.vis e e1)) (*)/\ (not (mem_key i l.l) <==> r.l = []*)))
                (decreases length l.l)
 
 #set-options "--z3rlimit 10000000"
 let project i l =
-    (A (fun o o1 -> (mem (get_id o, (i, get_op o)) l.l && mem (get_id o1, (i, get_op o1)) l.l &&  get_id o <> get_id o1 && l.vis (get_id o, (i, get_op o)) (get_id o1, (i, get_op o1)))) (project1 i l))
+    (A (fun o o1 -> (mem (get_id o, (Set i (get_op o))) l.l && mem (get_id o1, (Set i (get_op o1))) l.l && get_id o <> get_id o1 && l.vis (get_id o, (Set i (get_op o))) (get_id o1, (Set i (get_op o1))))) (project1 i l))
 
-val pre_cond_op_a : #st1:eqtype -> #o:eqtype -> {|mrdt st1 o|}
+val pre_cond_op_a : #st1:eqtype -> #o:eqtype -> #r:eqtype -> {|mrdt st1 o r|}
                   -> s1:s st1 -> op1:(nat * op o)
-                  -> Tot (b:bool {b = true <==> pre_cond_op #st1 #o (get_val_s #st1 #o (get_key op1) s1) (project_op op1)})
-let pre_cond_op_a #st1 #o s1 op = 
-    pre_cond_op #st1 #o (get_val_s #st1 #o (get_key op) s1) (project_op op)
+                  -> Tot (b:bool {b = true <==> pre_cond_op #st1 #o #r (get_val_s #st1 #o #r (get_key op1) s1) (project_op op1)})
+let pre_cond_op_a #st1 #o #r s1 op = 
+    pre_cond_op #st1 #o #r (get_val_s #st1 #o #r (get_key op) s1) (project_op op)
 
-val app_op_a : #st1:eqtype -> #o:eqtype -> {|mrdt st1 o|}
+val update : #st1:eqtype -> #o:eqtype -> #r:eqtype -> {|mrdt st1 o r|}
+           -> st:s st1
+           -> k:nat
+           -> v:st1
+           -> Pure (s st1)
+                  (requires mem_key_s k st)
+                  (ensures (fun res -> unique_key res /\ (forall e. mem_key_s e st <==> mem_key_s e res) /\
+                    (forall ch. ch <> k ==> (get_val_s #st1 #o #r ch st = get_val_s #st1 #o #r ch res))))
+#set-options "--z3rlimit 10000000"
+let rec update #st1 #o #r st k v = 
+  match st with
+  |(k1,v1)::xs -> if k = k1 then (k1,v)::xs else (k1,v1)::update #st1 #o #r xs k v
+
+val app_op_a : #st1:eqtype -> #o:eqtype -> #r:eqtype -> {|mrdt st1 o r|}
              -> st:s st1 -> op1:(nat * op o)
-             -> Pure (s st1)
-               (requires pre_cond_op_a #st1 #o st op1)
-               (ensures (fun r -> (forall ch. mem_key_s ch r <==> mem_key_s ch st \/ ch = get_key op1) /\ unique_key r /\
-                               (forall ch. ch <> get_key op1 ==> (get_val_s #st1 #o ch st = get_val_s #st1 #o ch r)) /\
-                             (get_val_s #st1 #o (get_key op1) r = 
-                                  (app_op #st1 #o (get_val_s #st1 #o (get_key op1) st) (project_op op1)))))
+             -> Pure ((s st1) * r)
+               (requires pre_cond_op_a #st1 #o #r st op1)
+               (ensures (fun res -> (opget op1 ==> (get_rval res = get_rval (app_op #st1 #o #r (get_val_s #st1 #o #r (get_key op1) st) (project_op op1))) /\ (get_st res = st)) /\
+                           (opset op1 ==> (get_rval res = get_rval (app_op #st1 #o #r (get_val_s #st1 #o #r (get_key op1) st) (project_op op1))) /\ (forall k. k <> get_key op1 ==> (get_val_s #st1 #o #r k st = get_val_s #st1 #o #r k (get_st res))) /\ (not (mem_key_s (get_key op1) st) ==> (forall e. mem e (get_st res) <==> mem e st \/ e = (get_key op1, (get_st ((app_op #st1 #o #r (get_val_s #st1 #o #r (get_key op1) st) (project_op op1))))))) /\
+               (mem_key_s (get_key op1) st ==> (forall e. mem e (get_st res) <==> mem e (update #st1 #o #r st (get_key op1) (get_st (app_op #st1 #o #r (get_val_s #st1 #o #r (get_key op1) st) (project_op op1)))))) /\
+                 (forall k. mem_key_s k (get_st res) <==> mem_key_s k st \/ k = get_key op1) /\ mem_key_s (get_key op1) (get_st res)) /\ unique_key (get_st res) (*)/\
+                   (opset op1 ==> (get_val_s #st1 #o #r (get_key op1) (get_st res) = 
+                         (get_st (app_op #st1 #o #r (get_val_s #st1 #o #r (get_key op1) st) (project_op op1))))*)))
 
 #set-options "--z3rlimit 10000000"
-let rec app_op_a #st1 #o st op1 =
+let rec app_op_a #st1 #o #r st op1 = 
+  (*)match op1 with
+  |(_, Get k ao) -> let (_, ret) = (app_op #st1 #o #r (get_val_s #st1 #o #r k st) (project_op op1)) in (st, ret)
+  |(_, Set k ao) -> let (v, ret) = (app_op #st1 #o #r (get_val_s #st1 #o #r k st) (project_op op1)) in (if mem_key_s (get_key op1) st then (update #st1 #o #r st (get_key op1) v, ret) else ((get_key op1, v)::st, ret))*)
   match st with
-  |[] -> [(get_key op1, (app_op (init #st1 #o) (project_op op1)))]
-  |(ch, x)::xs -> if ch = get_key op1 then (ch, (app_op x (project_op op1)))::xs
-                     else (ch, x)::app_op_a xs op1
+  |[] -> (match op1 with
+       |(_, Get k ao) -> let (_, ret) = (app_op #st1 #o #r (get_val_s #st1 #o #r k st) (project_op op1)) in 
+                            ((init_a), ret)
+       |(_, Set k ao) -> let (_, ret) = (app_op #st1 #o #r (get_val_s #st1 #o #r k st) (project_op op1)) in 
+                            ([(get_key op1, (get_st (app_op #st1 #o #r (init #st1 #o #r) (project_op op1))))], ret))
+  |(ch, x)::xs -> match op1 with
+                |(_, Get k ao) -> let (_, ret) = (app_op #st1 #o #r (get_val_s #st1 #o #r k st) (project_op op1)) in
+                                 (st, ret)
+                |(_, Set k ao) -> let (v, ret) = (app_op #st1 #o #r (get_val_s #st1 #o #r k st) (project_op op1)) in (if mem_key_s (get_key op1) st then (update #st1 #o #r st (get_key op1) v, ret) else ((get_key op1, v)::st, ret))
+
 
 val unique_keys : list nat -> Tot bool
 let rec unique_keys l =
@@ -144,57 +193,64 @@ let rec get_lst m =
   |[] -> []
   |(i,x)::xs -> i::get_lst xs
 
+val spec_a : #st:eqtype -> #o:eqtype -> #r:eqtype -> {|mrdt st o r|}
+           -> o1:(nat * (op o))
+           -> tr:ae (op o)
+           -> Pure r
+             (requires opget o1)
+             (ensures (fun res -> res = (spec #st #o #r) (project_op o1) (project (get_key o1) tr)))
+let spec_a #st #o #r o1 tr = (spec #st #o #r) (project_op o1) (project (get_key o1) tr)
+
 #set-options "--query_stats"
-val sim_a : #st:eqtype -> #o:eqtype -> {|mrdt st o|}
+val sim_a : #st:eqtype -> #o:eqtype -> #r:eqtype -> {|mrdt st o r|}
           -> tr:ae (op o)
           -> s1:s st
-          -> Tot (b:bool {(b = true) <==> (forall ch. mem_key_s ch s1 <==> mem_key ch tr.l) /\
-                          (forall ch. mem_key_s ch s1 ==> (sim #st #o) (project ch tr) (get_val_s #st #o ch s1)) /\
-                                     (forall e. mem e tr.l ==> (exists e1. mem e1 s1 /\ get_key e = get_key_s e1))})
+          -> Tot (b:bool {(b = true) <==> (forall k. mem_key_s k s1 ==> (exists e. mem e tr.l /\ get_id e = k /\ opset e)) /\
+            (forall k. mem_key_s k s1 ==> (sim #st #o #r) (project k tr) (get_val_s #st #o #r k s1)) /\
+            (forall e. mem e tr.l /\ opset e ==> (exists e1. mem e1 s1 /\ get_key e = get_key_s e1))})
 
 #set-options "--z3rlimit 10000000"
-let sim_a #st #o tr s1 =
-  forallb (fun e -> mem_key (get_key_s e) tr.l) s1 &&
-  forallb (fun e -> mem_key_s (get_key e) s1) tr.l &&
-  forallb (fun e -> (sim #st #o) (project (get_key_s e) tr) (get_val_s #st #o (get_key_s e) s1)) s1 &&
-  forallb (fun e -> (existsb (fun e1 -> get_key e = get_key_s e1) s1)) tr.l
+let sim_a #st #o #r tr s1 =
+  forallb (fun e -> (existsb (fun e1 -> get_id e1 = get_key_s e && opset e1) tr.l)) s1 &&
+  forallb (fun e -> (sim #st #o #r) (project (get_key_s e) tr) (get_val_s #st #o #r (get_key_s e) s1)) s1 &&
+  forallb (fun e -> (existsb (fun e1 -> get_key e = get_key_s e1) s1)) (filter (fun e -> opset e) tr.l)
 
-class alpha_map (st:eqtype) (o:eqtype) (m:mrdt st o) = {
+class alpha_map (st:eqtype) (o:eqtype) (r:eqtype) (m:mrdt st o r) = {
 
   lemma4 : tr:ae (op o) -> s1:s st
-         -> Lemma (requires sim_a tr s1)
-                 (ensures (forall i. (sim #st #o) (project i tr) (get_val_s #st #o i s1)));
+         -> Lemma (requires (sim_a #st #o #r) tr s1)
+                 (ensures (forall i. (sim #st #o #r) (project i tr) (get_val_s #st #o #r i s1)));
 
   lemma1 : tr:ae (op o)
          -> s1:s st
          -> op1:(nat * (op o))
-         -> Lemma (requires (sim_a tr s1) /\ (not (mem_id (get_id op1) tr.l)) /\
+         -> Lemma (requires ((sim_a #st #o #r) tr s1) /\ (not (mem_id (get_id op1) tr.l)) /\
                            (forall e. mem e tr.l ==> get_id e < get_id op1) /\ get_id op1 > 0 /\
-                           pre_cond_op #st #o (get_val_s #st #o (get_key op1) s1) (project_op op1))
-                 (ensures (forall i. mem_key_s i (app_op_a s1 op1) /\ i <> get_key op1 ==>
+                           pre_cond_op #st #o #r (get_val_s #st #o #r (get_key op1) s1) (project_op op1))
+                 (ensures (forall i. mem_key_s i (get_st (app_op_a #st #o #r s1 op1)) /\ i <> get_key op1 ==>
                    ((forall e. mem e (project i (append tr op1)).l <==> mem e (project i tr).l) /\
                    (forall e e1. mem e (project i (append tr op1)).l /\ mem e1 (project i (append tr op1)).l /\ 
                         get_id e <> get_id e1 /\ (project i (append tr op1)).vis e e1 <==> 
                  mem e (project i tr).l /\ mem e1 (project i tr).l /\ get_id e <> get_id e1 /\ (project i tr).vis e e1) /\
-                   (get_val_s #st #o i (app_op_a s1 op1) = (get_val_s #st #o i s1))) ==>
-                     (sim #st #o) (project i (append tr op1)) (get_val_s #st #o i (app_op_a s1 op1))));
+                   (get_val_s #st #o #r i (get_st (app_op_a #st #o #r s1 op1)) = (get_val_s #st #o #r i s1))) ==>
+                     (sim #st #o #r) (project i (append tr op1)) (get_val_s #st #o #r i (get_st (app_op_a #st #o #r s1 op1)))));
 
   lemma7 : tr:ae o -> s1:st -> tr1:ae o
-         -> Lemma (requires sim tr s1 /\ (forall e. mem e tr1.l <==> mem e tr.l) /\
+         -> Lemma (requires (sim #st #o #r) tr s1 /\ (forall e. mem e tr1.l <==> mem e tr.l) /\
                            (forall e e1. mem e tr1.l /\ mem e1 tr1.l /\ get_id e <> get_id e1 /\ tr1.vis e e1 <==>
                                     mem e tr.l /\ mem e1 tr.l /\ get_id e <> get_id e1 /\ tr.vis e e1))
-                 (ensures (sim tr1 s1));
+                 (ensures ((sim #st #o #r) tr1 s1));
 
   lemma2 : s1:s st
          -> Lemma (requires true)
-                 (ensures (forall e. mem e s1 ==> (get_val_s #st #o (get_key_s e) s1 = get_val_s1 #st e)))
+                 (ensures (forall e. mem e s1 ==> (get_val_s #st #o #r (get_key_s e) s1 = get_val_s1 #st e)))
 }
 
-val convergence_a1 : #st:eqtype -> #o:eqtype -> {| mrdt st o |} 
+val convergence_a1 : #st:eqtype -> #o:eqtype -> #r:eqtype -> {| mrdt st o r|} 
                    -> tr:ae (op o)
                    -> a:s st
                    -> b:s st
-                   -> Lemma (requires (sim_a tr a /\ sim_a tr b))
+                   -> Lemma (requires ((sim_a #st #o #r) tr a /\ (sim_a #st #o #r) tr b))
                          (ensures (forall e. mem_key_s e a <==> mem_key_s e b))
 let convergence_a1 tr a b = ()
 
@@ -203,8 +259,8 @@ val lem_oper1 : #o:eqtype
               -> op:(nat * (op o))
               -> Lemma (requires (not (mem_id (get_id op) tr.l)) /\
                                 (forall e. mem e tr.l ==> get_id e < get_id op) /\ get_id op > 0)
-                      (ensures (forall e. mem e (project (get_key op) (append tr op)).l <==> 
-                                     mem e (append (project (get_key op) tr) (project_op op)).l))
+                      (ensures (opset op ==> (forall e. mem e (project (get_key op) (append tr op)).l <==>
+                                      mem e (append (project (get_key op) tr) (project_op op)).l)))
 #set-options "--z3rlimit 10000000"
 let lem_oper1 tr op = ()
 
@@ -213,12 +269,12 @@ val lem_oper2 : #o:eqtype
               -> op:(nat * (op o))
               -> Lemma (requires (not (mem_id (get_id op) tr.l)) /\
                                 (forall e. mem e tr.l ==> get_id e < get_id op) /\ get_id op > 0)
-                      (ensures (forall e e1. mem e (project (get_key op) (append tr op)).l /\
+                      (ensures (opset op ==> (forall e e1. mem e (project (get_key op) (append tr op)).l /\
                         mem e1 (project (get_key op) (append tr op)).l /\ (get_id e <> get_id e1) /\
                         (project (get_key op) (append tr op)).vis e e1  <==> 
                         mem e (append (project (get_key op) tr) (project_op op)).l /\
                     mem e1 (append (project (get_key op) tr) (project_op op)).l /\ get_id e <> get_id e1 /\
-                        (append (project (get_key op) tr) (project_op op)).vis e e1))
+                        (append (project (get_key op) tr) (project_op op)).vis e e1)))
 #set-options "--z3rlimit 10000000"
 let lem_oper2 tr op = lem_oper1 tr op
 
@@ -241,14 +297,14 @@ val lem_oper : #o:eqtype
              -> op:(nat * (op o))
              -> Lemma (requires (not (mem_id (get_id op) tr.l)) /\
                                (forall e. mem e tr.l ==> get_id e < get_id op) /\ get_id op > 0)
-                     (ensures (forall e. mem e (project (get_key op) (append tr op)).l <==> 
+                     (ensures (opset op ==> (forall e. mem e (project (get_key op) (append tr op)).l <==> 
                                     mem e (append (project (get_key op) tr) (project_op op)).l) /\
                (forall e e1. mem e (project (get_key op) (append tr op)).l /\
                         mem e1 (project (get_key op) (append tr op)).l /\ (get_id e <> get_id e1) /\
                         (project (get_key op) (append tr op)).vis e e1  <==> 
                         mem e (append (project (get_key op) tr) (project_op op)).l /\
                     mem e1 (append (project (get_key op) tr) (project_op op)).l /\ get_id e <> get_id e1 /\
-                        (append (project (get_key op) tr) (project_op op)).vis e e1) /\
+                        (append (project (get_key op) tr) (project_op op)).vis e e1)) /\
          (forall i. i <> (get_key op) ==> (forall e. mem e (project i (append tr op)).l <==> mem e (project i tr).l) /\
          (forall e e1. mem e (project i (append tr op)).l /\ mem e1 (project i (append tr op)).l /\ get_id e <> get_id e1 /\
                     (project i (append tr op)).vis e e1 <==> 
@@ -260,64 +316,66 @@ let lem_oper tr op =
   lem_oper2 tr op;
   lem_oper3 tr op
 
-val prop_oper1 : #st1:eqtype -> #o:eqtype -> {|mrdt st1 o|} 
+val prop_oper1 : #st1:eqtype -> #o:eqtype -> #r:eqtype -> {|mrdt st1 o r|} 
                -> tr:ae (op o)
                -> st:s st1
                -> op1:(nat * (op o)) 
-               -> Lemma (requires (sim_a tr st) /\ (not (mem_id (get_id op1) tr.l)) /\
+               -> Lemma (requires (sim_a #st1 #o #r tr st) /\ (not (mem_id (get_id op1) tr.l)) /\
                                  (forall e. mem e tr.l ==> get_id e < get_id op1) /\ get_id op1 > 0 /\
-                                 pre_cond_op #st1 #o (get_val_s #st1 #o (get_key op1) st) (project_op op1))
-                       (ensures (forall ch. mem_key_s ch (app_op_a st op1) <==> mem_key ch (append tr op1).l))
+                                 pre_cond_op #st1 #o #r (get_val_s #st1 #o #r (get_key op1) st) (project_op op1))
+                       (ensures (forall e. mem e (append tr op1).l /\ opset e ==> (exists e1. mem e1 (get_st (app_op_a #st1 #o #r st op1)) /\ get_key e = get_key_s e1)))
+
 #set-options "--z3rlimit 10000000"
 let prop_oper1 tr st op = lem_oper tr op
 
-val prop_oper2 : #st1:eqtype -> #o:eqtype -> {|mrdt st1 o|} 
+val prop_oper2 : #st1:eqtype -> #o:eqtype -> #r:eqtype -> {|mrdt st1 o r|} 
                -> tr:ae (op o)
                -> st:s st1
                -> op1:(nat * (op o)) 
-               -> Lemma (requires (sim_a tr st) /\ (not (mem_id (get_id op1) tr.l)) /\
+               -> Lemma (requires (sim_a #st1 #o #r tr st) /\ (not (mem_id (get_id op1) tr.l)) /\
                                  (forall e. mem e tr.l ==> get_id e < get_id op1) /\ get_id op1 > 0 /\
-                                 pre_cond_op #st1 #o (get_val_s #st1 #o (get_key op1) st) (project_op op1))
-                       (ensures (forall e. mem e (append tr op1).l ==> (exists e1. mem e1 (app_op_a st op1) /\ get_key e = get_key_s e1)))
+                                 pre_cond_op #st1 #o #r (get_val_s #st1 #o #r (get_key op1) st) (project_op op1) /\
+                                 ((sim #st1 #o #r) (project (get_key op1) (append tr op1)) (get_val_s #st1 #o #r (get_key op1) (get_st (app_op_a #st1 #o #r st op1)))))
+                       (ensures (forall k. mem_key_s k (get_st (app_op_a #st1 #o #r st op1)) ==> (exists e. mem e (append tr op1).l /\ get_id e = k /\ opset e)))
 
 #set-options "--z3rlimit 10000000"
-let prop_oper2 tr st op = 
+let prop_oper2 #st1 #o #r tr st op = admit();
   lem_oper tr op;
-  prop_oper1 tr st op
+  prop_oper1 #st1 #o #r tr st op
 
-val prop_oper3 : #st1:eqtype -> #o:eqtype -> #m:(mrdt st1 o) -> {|alpha_map st1 o m|}
+val prop_oper3 : #st1:eqtype -> #o:eqtype -> #r:eqtype -> #m:(mrdt st1 o r) -> {|alpha_map st1 o r m|}
                -> tr:ae (op o)
                -> st:s st1
                -> op1:(nat * (op o)) 
-               -> Lemma (requires (sim_a tr st) /\ (not (mem_id (get_id op1) tr.l)) /\
+               -> Lemma (requires (sim_a #st1 #o #r tr st) /\ (not (mem_id (get_id op1) tr.l)) /\
                                  (forall e. mem e tr.l ==> get_id e < get_id op1) /\ get_id op1 > 0 /\
-                                 pre_cond_op #st1 #o (get_val_s #st1 #o (get_key op1) st) (project_op op1))
-                       (ensures (forall ch. mem_key_s ch (app_op_a st op1) /\ ch <> get_key op1 ==>
-                         (sim #st1 #o) (project ch (append tr op1)) (get_val_s #st1 #o ch (app_op_a st op1))))
+                                 pre_cond_op #st1 #o #r (get_val_s #st1 #o #r (get_key op1) st) (project_op op1))
+                       (ensures (forall ch. mem_key_s ch (get_st (app_op_a #st1 #o #r st op1)) /\ ch <> get_key op1 ==>
+   (sim #st1 #o #r) (project ch (append tr op1)) (get_val_s #st1 #o #r ch (get_st (app_op_a #st1 #o #r st op1)))))
 
 #set-options "--z3rlimit 10000000"
-let prop_oper3 #st1 #o #m tr st op = 
+let prop_oper3 #st1 #o #r #m tr st op = 
   lem_oper tr op;
-  prop_oper1 tr st op;
-  prop_oper2 tr st op;
-  lemma1 #st1 #o #m tr st op
+  prop_oper1 #st1 #o #r tr st op;
+  prop_oper2 #st1 #o #r tr st op;
+  lemma1 #st1 #o #r #m tr st op
 
-val prop_oper_a : #st1:eqtype -> #o:eqtype -> #m:(mrdt st1 o) -> {|alpha_map st1 o m|}
+val prop_oper_a : #st1:eqtype -> #o:eqtype -> #r:eqtype -> #m:(mrdt st1 o r) -> {|alpha_map st1 o r m|}
                 -> tr:ae (op o)
                 -> st:s st1
                 -> op1:(nat * (op o)) 
-                -> Lemma (requires (sim_a tr st) /\ (not (mem_id (get_id op1) tr.l)) /\
+                -> Lemma (requires (sim_a #st1 #o #r tr st) /\ (not (mem_id (get_id op1) tr.l)) /\
                                   (forall e. mem e tr.l ==> get_id e < get_id op1) /\ get_id op1 > 0 /\
-                                  pre_cond_op #st1 #o (get_val_s #st1 #o (get_key op1) st) (project_op op1) /\
-     ((sim #st1 #o) (project (get_key op1) (append tr op1)) (get_val_s #st1 #o (get_key op1) (app_op_a st op1))))
-                      (ensures (sim_a (append tr op1) (app_op_a st op1)))
+                                  pre_cond_op #st1 #o #r (get_val_s #st1 #o #r (get_key op1) st) (project_op op1) /\
+     ((sim #st1 #o #r) (project (get_key op1) (append tr op1)) (get_val_s #st1 #o #r (get_key op1) (get_st (app_op_a #st1 #o #r st op1)))))
+                      (ensures (sim_a #st1 #o #r (append tr op1) (get_st (app_op_a #st1 #o #r st op1))))
 
 #set-options "--z3rlimit 10000000"
-let prop_oper_a #st1 #o #m tr st op = 
+let prop_oper_a #st1 #o #r #m tr st op = 
   lem_oper tr op;
-  prop_oper1 tr st op;
-  prop_oper2 tr st op;
-  prop_oper3 #st1 #o #m tr st op
+  prop_oper1 #st1 #o #r tr st op;
+  prop_oper2 #st1 #o #r tr st op;
+  prop_oper3 #st1 #o #r #m tr st op
 
 val get_key_lst : #st:eqtype 
                 -> l:s st -> a:s st -> b:s st
@@ -333,15 +391,15 @@ let rec get_key_lst #st l a b =
   |[],x::xs,_ -> if (mem_key_s (get_key_s x) b) then get_key_lst [] xs b else (get_key_s x)::(get_key_lst [] xs b)
   |[],[],x::xs -> (get_key_s x)::(get_key_lst [] [] xs)
 
-val pre_cond_merge1_a : #st:eqtype -> #o:eqtype -> {|mrdt st o|}
+val pre_cond_merge1_a : #st:eqtype -> #o:eqtype -> #r:eqtype -> {|mrdt st o r|}
                       -> l:s st -> a:s st -> b:s st 
                       -> Tot (b1:bool {b1=true <==> (forall e. mem_key_s e l ==> mem_key_s e a /\ mem_key_s e b) /\
                         (forall ch. mem_key_s ch a \/ mem_key_s ch b ==> 
-                pre_cond_merge1 #st #o (get_val_s #st #o ch l) (get_val_s #st #o ch a) (get_val_s #st #o ch b))})
-let pre_cond_merge1_a #st #o l a b =
+                pre_cond_merge1 #st #o #r (get_val_s #st #o #r ch l) (get_val_s #st #o #r ch a) (get_val_s #st #o #r ch b))})
+let pre_cond_merge1_a #st #o #r l a b =
   forallb (fun e -> mem_key_s (get_key_s #st e) a && mem_key_s (get_key_s #st e) b) l &&
-  forallb (fun ch -> pre_cond_merge1 #st #o (get_val_s #st #o ch l) 
-             (get_val_s #st #o ch a) (get_val_s #st #o ch b)) (get_key_lst l a b)
+  forallb (fun ch -> pre_cond_merge1 #st #o #r (get_val_s #st #o #r ch l) 
+             (get_val_s #st #o #r ch a) (get_val_s #st #o #r ch b)) (get_key_lst l a b)
 
 val remove_key : #st:eqtype 
                -> ch:nat
@@ -354,41 +412,41 @@ let rec remove_key #st ch a =
   match a with
   |(ch1,v)::xs -> if ch = ch1 then xs else (ch1,v)::remove_key ch xs
 
-val merge2 : #st:eqtype -> #o:eqtype -> {|mrdt st o|}
+val merge2 : #st:eqtype -> #o:eqtype -> #r:eqtype -> {|mrdt st o r|}
            -> l:s st
            -> a:s st
            -> b:s st
            -> lst:list nat
            -> Pure (s st)
-                (requires pre_cond_merge1_a #st #o l a b /\ unique_keys lst /\
+                (requires pre_cond_merge1_a #st #o #r l a b /\ unique_keys lst /\
                           (forall ch. mem ch lst ==> mem_key_s ch a \/ mem_key_s ch b))
-                (ensures (fun r -> (forall ch. mem_key_s ch r <==> mem ch lst) /\ unique_key r /\
-                         (forall ch. mem ch lst ==> (get_val_s #st #o ch r) =
-                         (merge1 #st #o (get_val_s #st #o ch l) (get_val_s #st #o ch a) (get_val_s #st #o ch b)))))
+                (ensures (fun res -> (forall ch. mem_key_s ch res <==> mem ch lst) /\ unique_key res /\
+                         (forall ch. mem ch lst ==> (get_val_s #st #o #r ch res) =
+                         (merge1 #st #o #r (get_val_s #st #o #r ch l) (get_val_s #st #o #r ch a) (get_val_s #st #o #r ch b)))))
                 (decreases lst)
 
 #set-options "--z3rlimit 10000000" 
-let rec merge2 #st #o l a b lst =
+let rec merge2 #st #o #r l a b lst =
   match lst with
   |[] -> []
-  |x::xs -> (x, merge1 #st #o (get_val_s #st #o x l) (get_val_s #st #o x a) (get_val_s #st #o x b))::merge2 #st #o l a b xs
+  |x::xs -> (x, merge1 #st #o #r (get_val_s #st #o #r x l) (get_val_s #st #o #r x a) (get_val_s #st #o #r x b))::merge2 #st #o #r l a b xs
 
-val merge1_a : #st:eqtype -> #o:eqtype -> {|mrdt st o|}
+val merge1_a : #st:eqtype -> #o:eqtype -> #r:eqtype -> {|mrdt st o r|}
              -> l:s st
              -> a:s st
              -> b:s st
              -> Pure (s st)
-               (requires pre_cond_merge1_a #st #o l a b)
-               (ensures (fun r -> (forall ch. mem_key_s ch r <==> mem_key_s ch a \/ mem_key_s ch b) /\ unique_key r /\
-                               (forall ch. mem_key_s ch a \/ mem_key_s ch b ==> (get_val_s #st #o ch r) =
-                      (merge1 #st #o (get_val_s #st #o ch l) (get_val_s #st #o ch a) (get_val_s #st #o ch b)))))
+               (requires pre_cond_merge1_a #st #o #r l a b)
+               (ensures (fun res -> (forall ch. mem_key_s ch res <==> mem_key_s ch a \/ mem_key_s ch b) /\ unique_key res /\
+                               (forall ch. mem_key_s ch a \/ mem_key_s ch b ==> (get_val_s #st #o #r ch res) =
+                      (merge1 #st #o #r (get_val_s #st #o #r ch l) (get_val_s #st #o #r ch a) (get_val_s #st #o #r ch b)))))
 
 #set-options "--z3rlimit 10000000" 
-let merge1_a #st #o l a b = 
+let merge1_a #st #o #r l a b = 
  let lst = get_key_lst l a b in
- merge2 #st #o l a b lst
+ merge2 #st #o #r l a b lst
 
-val lem_merge1 : #st:eqtype -> #o:eqtype -> {|mrdt st o|}
+val lem_merge1 : #st:eqtype -> #o:eqtype -> #r:eqtype -> {|mrdt st o r|}
                -> ltr:ae (op o)
                -> l:s st
                -> atr:ae (op o)
@@ -399,19 +457,19 @@ val lem_merge1 : #st:eqtype -> #o:eqtype -> {|mrdt st o|}
                -> Lemma (requires (forall e. mem e ltr.l ==> not (mem_id (get_id e) atr.l)) /\
                                  (forall e. mem e atr.l ==> not (mem_id (get_id e) btr.l)) /\
                                  (forall e. mem e ltr.l ==> not (mem_id (get_id e) btr.l)) /\
-                                 (sim_a ltr l /\ sim_a (union ltr atr) a /\ sim_a (union ltr btr) b) /\
+               (sim_a #st #o #r ltr l /\ sim_a #st #o #r (union ltr atr) a /\ sim_a #st #o #r (union ltr btr) b) /\
                                  (forall ch. mem ch lst <==> mem_key_s ch a \/ mem_key_s ch b) /\ unique_keys lst)
                        (ensures (forall i. mem_key_s i l ==> mem_key_s i a /\ mem_key_s i b))
 
 #set-options "--z3rlimit 10000000"
 let lem_merge1 ltr l atr a btr b lst = ()
 
-val pre_cond_merge_a : #st:eqtype -> #o:eqtype -> {|mrdt st o|}
+val pre_cond_merge_a : #st:eqtype -> #o:eqtype -> #r:eqtype -> {|mrdt st o r|}
             -> ltr:ae (op o) -> l:s st -> atr:ae (op o) -> a:s st -> btr:ae (op o) -> b:s st
             -> Tot bool
 let pre_cond_merge_a ltr l atr a btr b = true
 
-val merge_a : #st:eqtype -> #o:eqtype -> {|mrdt st o|}
+val merge_a : #st:eqtype -> #o:eqtype -> #r:eqtype -> {|mrdt st o r|}
             -> ltr:ae (op o)
             -> l:s st
             -> atr:ae (op o)
@@ -422,27 +480,28 @@ val merge_a : #st:eqtype -> #o:eqtype -> {|mrdt st o|}
               (requires (forall e. mem e ltr.l ==> not (mem_id (get_id e) atr.l)) /\
                         (forall e. mem e atr.l ==> not (mem_id (get_id e) btr.l)) /\
                         (forall e. mem e ltr.l ==> not (mem_id (get_id e) btr.l)) /\
-                        (sim_a ltr l /\ sim_a (union ltr atr) a /\ sim_a (union ltr btr) b) /\ pre_cond_merge1_a #st #o l a b /\
+                   (sim_a #st #o #r ltr l /\ sim_a #st #o #r (union ltr atr) a /\ sim_a #st #o #r (union ltr btr) b) /\ 
+                        pre_cond_merge1_a #st #o #r l a b /\
                         (forall ch. mem_key_s ch a \/ mem_key_s ch b ==> 
-                        (pre_cond_merge #st #o (project ch ltr) (get_val_s #st #o ch l)
-                                               (project ch atr) (get_val_s #st #o ch a)
-                                               (project ch btr) (get_val_s #st #o ch b)) /\
+                        (pre_cond_merge #st #o #r (project ch ltr) (get_val_s #st #o #r ch l)
+                                                  (project ch atr) (get_val_s #st #o #r ch a)
+                                                  (project ch btr) (get_val_s #st #o #r ch b)) /\
                         (forall e. mem e (project ch ltr).l ==> not (mem_id (get_id e) (project ch atr).l)) /\
                         (forall e. mem e (project ch atr).l ==> not (mem_id (get_id e) (project ch btr).l)) /\
                         (forall e. mem e (project ch ltr).l ==> not (mem_id (get_id e) (project ch btr).l)) /\
-                        (sim #st #o (project ch ltr) (get_val_s #st #o ch l) /\ sim #st #o (union (project ch ltr) (project ch atr)) (get_val_s #st #o ch a) /\ sim #st #o (union (project ch ltr) (project ch btr)) (get_val_s #st #o ch b))))
+                        (sim #st #o #r (project ch ltr) (get_val_s #st #o #r ch l) /\ sim #st #o #r (union (project ch ltr) (project ch atr)) (get_val_s #st #o #r ch a) /\ sim #st #o #r (union (project ch ltr) (project ch btr)) (get_val_s #st #o #r ch b))))
 
-              (ensures (fun r -> (forall i. mem_key_s i l ==> mem_key_s i a /\ mem_key_s i b) /\
-                              (forall i. mem_key_s i r <==> mem_key_s i a \/ mem_key_s i b) /\
-                              (forall ch. mem_key_s ch r ==> (get_val_s #st #o ch r) =
-                    (merge1 #st #o (get_val_s #st #o ch l) (get_val_s #st #o ch a) (get_val_s #st #o ch b))) /\
-                         (forall ch. mem_key_s ch r ==> (get_val_s #st #o ch r) =
-                  (merge #st #o (project ch ltr) (get_val_s #st #o ch l) (project ch atr) (get_val_s #st #o ch a) (project ch btr) (get_val_s #st #o ch b))) /\ (r = merge1_a #st #o l a b)))
+              (ensures (fun res -> (forall i. mem_key_s i l ==> mem_key_s i a /\ mem_key_s i b) /\
+                              (forall i. mem_key_s i res <==> mem_key_s i a \/ mem_key_s i b) /\
+                              (forall ch. mem_key_s ch res ==> (get_val_s #st #o #r ch res) =
+                    (merge1 #st #o #r (get_val_s #st #o #r ch l) (get_val_s #st #o #r ch a) (get_val_s #st #o #r ch b))) /\
+                         (forall ch. mem_key_s ch res ==> (get_val_s #st #o #r ch res) =
+                  (merge #st #o #r (project ch ltr) (get_val_s #st #o #r ch l) (project ch atr) (get_val_s #st #o #r ch a) (project ch btr) (get_val_s #st #o #r ch b))) /\ (res = merge1_a #st #o #r l a b)))
 
-let merge_a #st #o ltr l atr a btr b = 
+let merge_a #st #o #r ltr l atr a btr b = 
   let keys = get_key_lst l a b in
-  lem_merge1 ltr l atr a btr b keys;
-  let r = merge1_a #st #o l a b in
+  lem_merge1 #st #o #r ltr l atr a btr b keys;
+  let r = merge1_a #st #o #r l a b in
   r
 
 val lemma6 : #o:eqtype 
@@ -514,7 +573,7 @@ val lemma9 : #o:eqtype
 #set-options "--z3rlimit 10000000"
 let lemma9 #o ltr atr btr = ()
 
-val prop_merge1 : #st:eqtype -> #o:eqtype -> #m:(mrdt st o) -> {|alpha_map st o m|}
+val prop_merge1 : #st:eqtype -> #o:eqtype -> #r:eqtype -> #m:(mrdt st o r) -> {|alpha_map st o r m|}
                 -> ltr:ae (op o)
                 -> l:s st
                 -> atr:ae (op o)
@@ -528,41 +587,41 @@ val prop_merge1 : #st:eqtype -> #o:eqtype -> #m:(mrdt st o) -> {|alpha_map st o 
                                   (forall i e. mem e (project i ltr).l ==> not (mem_id (get_id e) (project i atr).l)) /\
                                   (forall i e. mem e (project i atr).l ==> not (mem_id (get_id e) (project i btr).l)) /\
                                   (forall i e. mem e (project i ltr).l ==> not (mem_id (get_id e) (project i btr).l)) /\
-                                  (sim_a ltr l /\ sim_a (union ltr atr) a /\ sim_a (union ltr btr) b) /\
+                    (sim_a #st #o #r ltr l /\ sim_a #st #o #r (union ltr atr) a /\ sim_a #st #o #r (union ltr btr) b) /\
                                   (forall i. mem_key_s i l ==> mem_key_s i a /\ mem_key_s i b) /\
                                   (forall i. mem i chs ==> mem_key_s i a \/ mem_key_s i b) /\
-                                  pre_cond_merge1_a #st #o l a b /\
+                                  pre_cond_merge1_a #st #o #r l a b /\
                                   (forall i. mem_key_s i a \/ mem_key_s i b ==> 
-                                  pre_cond_merge #st #o (project i ltr) (get_val_s #st #o i l)
-                                                           (project i atr) (get_val_s #st #o i a)
-                                                           (project i btr) (get_val_s #st #o i b) /\
+                                  pre_cond_merge #st #o #r (project i ltr) (get_val_s #st #o #r i l)
+                                                           (project i atr) (get_val_s #st #o #r i a)
+                                                           (project i btr) (get_val_s #st #o #r i b) /\
                                   (forall e. mem e (project i ltr).l ==> not (mem_id (get_id e) (project i atr).l)) /\
                                   (forall e. mem e (project i atr).l ==> not (mem_id (get_id e) (project i btr).l)) /\
                                   (forall e. mem e (project i ltr).l ==> not (mem_id (get_id e) (project i btr).l)) /\
-                                  (sim #st #o (project i ltr) (get_val_s #st #o i l) /\ sim #st #o (union (project i ltr) (project i atr)) (get_val_s #st #o i a) /\ sim #st #o (union (project i ltr) (project i btr)) (get_val_s #st #o i b))) /\
-                                  (forall i. mem i chs ==> mem_key_s i (merge_a ltr l atr a btr b)))
+                                  (sim #st #o #r (project i ltr) (get_val_s #st #o #r i l) /\ sim #st #o #r (union (project i ltr) (project i atr)) (get_val_s #st #o #r i a) /\ sim #st #o #r (union (project i ltr) (project i btr)) (get_val_s #st #o #r i b))) /\
+                                  (forall i. mem i chs ==> mem_key_s i (merge_a #st #o #r ltr l atr a btr b)))
                         (ensures (forall i. mem i chs ==> 
-             ((sim #st #o) (project i (absmerge ltr atr btr)) (get_val_s #st #o i (merge_a ltr l atr a btr b)))))
+             ((sim #st #o #r) (project i (absmerge ltr atr btr)) (get_val_s #st #o #r i (merge_a #st #o #r ltr l atr a btr b)))))
                         (decreases chs)
 
 #set-options "--z3rlimit 10000000"
-let rec prop_merge1 #st #o #m ltr l atr a btr b lst =
+let rec prop_merge1 #st #o #r #m ltr l atr a btr b lst =
   match lst with
   |[] -> ()
-  |i::is -> lemma4 #st #o #m ltr l; lemma4 #st #o #m (union ltr atr) a; lemma4 #st #o #m (union ltr btr) b;
+  |i::is -> lemma4 #st #o #r #m ltr l; lemma4 #st #o #r #m (union ltr atr) a; lemma4 #st #o #r #m (union ltr btr) b;
           lemma8 #o ltr atr; lemma8 #o ltr btr; 
-          lemma7 #st #o #m (project i (union ltr atr)) (get_val_s #st #o i a) (union (project i ltr) (project i atr));
-          lemma7 #st #o #m (project i (union ltr btr)) (get_val_s #st #o i b) (union (project i ltr) (project i btr));
-          (prop_merge #st #o) (project i ltr) (get_val_s #st #o i l) (project i atr) (get_val_s #st #o i a) (project i btr) (get_val_s #st #o i b);
-          assert (sim #st #o (absmerge (project i ltr) (project i atr) (project i btr)) (merge #st #o (project i ltr) (get_val_s #st #o i l) (project i atr) (get_val_s #st #o i a) (project i btr) (get_val_s #st #o i b)));
+          lemma7 #st #o #r #m (project i (union ltr atr)) (get_val_s #st #o #r i a) (union (project i ltr) (project i atr));
+          lemma7 #st #o #r #m (project i (union ltr btr)) (get_val_s #st #o #r i b) (union (project i ltr) (project i btr));
+          (prop_merge #st #o #r) (project i ltr) (get_val_s #st #o #r i l) (project i atr) (get_val_s #st #o #r i a) (project i btr) (get_val_s #st #o #r i b);
+          assert (sim #st #o #r (absmerge (project i ltr) (project i atr) (project i btr)) (merge #st #o #r (project i ltr) (get_val_s #st #o #r i l) (project i atr) (get_val_s #st #o #r i a) (project i btr) (get_val_s #st #o #r i b)));
           lemma9 #o ltr atr btr;
-          assert ((sim #st #o) (absmerge (project i ltr) (project i atr) (project i btr)) (get_val_s #st #o i (merge_a ltr l atr a btr b))); 
-          lemma7 #st #o #m (absmerge (project i ltr) (project i atr) (project i btr)) 
-                 (get_val_s #st #o i (merge_a ltr l atr a btr b)) (project i (absmerge ltr atr btr)); 
-          assert ((sim #st #o) (project i (absmerge ltr atr btr)) (get_val_s #st #o i (merge_a ltr l atr a btr b)));
-          prop_merge1 #st #o #m ltr l atr a btr b is
+          assert ((sim #st #o #r) (absmerge (project i ltr) (project i atr) (project i btr)) (get_val_s #st #o #r i (merge_a #st #o #r ltr l atr a btr b))); 
+          lemma7 #st #o #r #m (absmerge (project i ltr) (project i atr) (project i btr)) 
+                   (get_val_s #st #o #r i (merge_a #st #o #r ltr l atr a btr b)) (project i (absmerge ltr atr btr)); 
+          assert ((sim #st #o #r) (project i (absmerge ltr atr btr)) (get_val_s #st #o #r i (merge_a #st #o #r ltr l atr a btr b)));
+          prop_merge1 #st #o #r #m ltr l atr a btr b is
 
-val prop_merge21 : #st:eqtype -> #o:eqtype -> #m:(mrdt st o) -> {|alpha_map st o m|}
+val prop_merge21 : #st:eqtype -> #o:eqtype -> #r:eqtype -> #m:(mrdt st o r) -> {|alpha_map st o r m|}
           -> ltr:ae (op o)
           -> l:s st
           -> atr:ae (op o)
@@ -572,25 +631,25 @@ val prop_merge21 : #st:eqtype -> #o:eqtype -> #m:(mrdt st o) -> {|alpha_map st o
           -> Lemma (requires (forall e. mem e ltr.l ==> not (mem_id (get_id e) atr.l)) /\
                             (forall e. mem e atr.l ==> not (mem_id (get_id e) btr.l)) /\
                             (forall e. mem e ltr.l ==> not (mem_id (get_id e) btr.l)) /\
-                            (sim_a ltr l /\ sim_a (union ltr atr) a /\ sim_a (union ltr btr) b) /\
-                             pre_cond_merge1_a #st #o l a b /\
+                            (sim_a #st #o #r ltr l /\ sim_a #st #o #r (union ltr atr) a /\ sim_a #st #o #r (union ltr btr) b) /\
+                             pre_cond_merge1_a #st #o #r l a b /\
                             (forall ch. mem_key_s ch a \/ mem_key_s ch b ==> 
-                            (pre_cond_merge #st #o (project ch ltr) (get_val_s #st #o ch l)
-                                                   (project ch atr) (get_val_s #st #o ch a)
-                                                   (project ch btr) (get_val_s #st #o ch b)) /\
+                            (pre_cond_merge #st #o #r (project ch ltr) (get_val_s #st #o #r ch l)
+                                                      (project ch atr) (get_val_s #st #o #r ch a)
+                                                      (project ch btr) (get_val_s #st #o #r ch b)) /\
                             (forall e. mem e (project ch ltr).l ==> not (mem_id (get_id e) (project ch atr).l)) /\
                             (forall e. mem e (project ch atr).l ==> not (mem_id (get_id e) (project ch btr).l)) /\
                             (forall e. mem e (project ch ltr).l ==> not (mem_id (get_id e) (project ch btr).l)) /\
-                            (sim #st #o (project ch ltr) (get_val_s #st #o ch l) /\ sim #st #o (union (project ch ltr) (project ch atr)) (get_val_s #st #o ch a) /\ sim #st #o (union (project ch ltr) (project ch btr)) (get_val_s #st #o ch b))))
-                  (ensures (forall e. mem e (merge_a ltr l atr a btr b) ==> mem_key (get_key_s e) (absmerge ltr atr btr).l))
+                            (sim #st #o #r (project ch ltr) (get_val_s #st #o #r ch l) /\ sim #st #o #r (union (project ch ltr) (project ch atr)) (get_val_s #st #o #r ch a) /\ sim #st #o #r (union (project ch ltr) (project ch btr)) (get_val_s #st #o #r ch b))))
+                  (ensures (forall k. mem_key_s k (merge_a #st #o #r ltr l atr a btr b) ==> (exists e. mem e (absmerge ltr atr btr).l /\ get_id e = k /\ opset e)))
 
 #set-options "--z3rlimit 10000000"
-let prop_merge21 #st #o #m ltr l atr a btr b = 
-  lemma2 #st #o #m (merge_a ltr l atr a btr b);
+let prop_merge21 #st #o #r #m ltr l atr a btr b = 
+  lemma2 #st #o #r #m (merge_a #st #o #r ltr l atr a btr b);
   lemma6 ltr atr; lemma6 ltr btr;
   lemma61 ltr atr btr
 
-val prop_merge22 : #st:eqtype -> #o:eqtype -> #m:(mrdt st o) -> {|alpha_map st o m|}
+val prop_merge22 : #st:eqtype -> #o:eqtype -> #r:eqtype -> #m:(mrdt st o r) -> {|alpha_map st o r m|}
           -> ltr:ae (op o)
           -> l:s st
           -> atr:ae (op o)
@@ -600,26 +659,25 @@ val prop_merge22 : #st:eqtype -> #o:eqtype -> #m:(mrdt st o) -> {|alpha_map st o
           -> Lemma (requires (forall e. mem e ltr.l ==> not (mem_id (get_id e) atr.l)) /\
                             (forall e. mem e atr.l ==> not (mem_id (get_id e) btr.l)) /\
                             (forall e. mem e ltr.l ==> not (mem_id (get_id e) btr.l)) /\
-                            (sim_a ltr l /\ sim_a (union ltr atr) a /\ sim_a (union ltr btr) b) /\
-                             pre_cond_merge1_a #st #o l a b /\
+                            (sim_a #st #o #r ltr l /\ sim_a #st #o #r (union ltr atr) a /\ sim_a #st #o #r (union ltr btr) b) /\
+                             pre_cond_merge1_a #st #o #r l a b /\
                             (forall ch. mem_key_s ch a \/ mem_key_s ch b ==> 
-                            (pre_cond_merge #st #o (project ch ltr) (get_val_s #st #o ch l)
-                                                   (project ch atr) (get_val_s #st #o ch a)
-                                                   (project ch btr) (get_val_s #st #o ch b)) /\
+                            (pre_cond_merge #st #o #r (project ch ltr) (get_val_s #st #o #r ch l)
+                                                      (project ch atr) (get_val_s #st #o #r ch a)
+                                                      (project ch btr) (get_val_s #st #o #r ch b)) /\
                             (forall e. mem e (project ch ltr).l ==> not (mem_id (get_id e) (project ch atr).l)) /\
                             (forall e. mem e (project ch atr).l ==> not (mem_id (get_id e) (project ch btr).l)) /\
                             (forall e. mem e (project ch ltr).l ==> not (mem_id (get_id e) (project ch btr).l)) /\
-                            (sim #st #o (project ch ltr) (get_val_s #st #o ch l) /\ sim #st #o (union (project ch ltr) (project ch atr)) (get_val_s #st #o ch a) /\ sim #st #o (union (project ch ltr) (project ch btr)) (get_val_s #st #o ch b))))
-                   (ensures (forall e. mem e (absmerge ltr atr btr).l ==> 
-                                      mem_key_s (get_key e) (merge_a ltr l atr a btr b)))
+                            (sim #st #o #r (project ch ltr) (get_val_s #st #o #r ch l) /\ sim #st #o #r (union (project ch ltr) (project ch atr)) (get_val_s #st #o #r ch a) /\ sim #st #o #r (union (project ch ltr) (project ch btr)) (get_val_s #st #o #r ch b))))
+                  (ensures (forall e. mem e (absmerge ltr atr btr).l /\ opset e ==> (exists e1. mem e1 (merge_a #st #o #r ltr l atr a btr b) /\ get_key e = get_key_s e1)))
 
 #set-options "--z3rlimit 10000000"
-let prop_merge22 #st #o #m ltr l atr a btr b = 
-  lemma2 #st #o #m (merge_a ltr l atr a btr b);
+let prop_merge22 #st #o #r #m ltr l atr a btr b = 
+  lemma2 #st #o #r #m (merge_a #st #o #r ltr l atr a btr b);
   lemma6 ltr atr; lemma6 ltr btr;
   lemma61 ltr atr btr
 
-val prop_merge2 : #st:eqtype -> #o:eqtype -> #m:(mrdt st o) -> {|alpha_map st o m|}
+val prop_merge_a : #st:eqtype -> #o:eqtype -> #r:eqtype -> #m:(mrdt st o r) -> {|alpha_map st o r m|}
           -> ltr:ae (op o)
           -> l:s st
           -> atr:ae (op o)
@@ -629,80 +687,32 @@ val prop_merge2 : #st:eqtype -> #o:eqtype -> #m:(mrdt st o) -> {|alpha_map st o 
           -> Lemma (requires (forall e. mem e ltr.l ==> not (mem_id (get_id e) atr.l)) /\
                             (forall e. mem e atr.l ==> not (mem_id (get_id e) btr.l)) /\
                             (forall e. mem e ltr.l ==> not (mem_id (get_id e) btr.l)) /\
-                            (sim_a ltr l /\ sim_a (union ltr atr) a /\ sim_a (union ltr btr) b) /\
-                             pre_cond_merge1_a #st #o l a b /\
+                            (sim_a #st #o #r ltr l /\ sim_a #st #o #r (union ltr atr) a /\ sim_a #st #o #r (union ltr btr) b) /\
+                             pre_cond_merge1_a #st #o #r l a b /\
                             (forall ch. mem_key_s ch a \/ mem_key_s ch b ==> 
-                            (pre_cond_merge #st #o (project ch ltr) (get_val_s #st #o ch l)
-                                                   (project ch atr) (get_val_s #st #o ch a)
-                                                   (project ch btr) (get_val_s #st #o ch b)) /\
+                            (pre_cond_merge #st #o #r (project ch ltr) (get_val_s #st #o #r ch l)
+                                                      (project ch atr) (get_val_s #st #o #r ch a)
+                                                      (project ch btr) (get_val_s #st #o #r ch b)) /\
                             (forall e. mem e (project ch ltr).l ==> not (mem_id (get_id e) (project ch atr).l)) /\
                             (forall e. mem e (project ch atr).l ==> not (mem_id (get_id e) (project ch btr).l)) /\
                             (forall e. mem e (project ch ltr).l ==> not (mem_id (get_id e) (project ch btr).l)) /\
-                            (sim #st #o (project ch ltr) (get_val_s #st #o ch l) /\ sim #st #o (union (project ch ltr) (project ch atr)) (get_val_s #st #o ch a) /\ sim #st #o (union (project ch ltr) (project ch btr)) (get_val_s #st #o ch b))))
-                   (ensures (forall ch. mem_key_s ch (merge_a ltr l atr a btr b) <==> 
-                                       mem_key ch (absmerge ltr atr btr).l))
+                            (sim #st #o #r (project ch ltr) (get_val_s #st #o #r ch l) /\ sim #st #o #r (union (project ch ltr) (project ch atr)) (get_val_s #st #o #r ch a) /\ sim #st #o #r (union (project ch ltr) (project ch btr)) (get_val_s #st #o #r ch b))))
+                 (ensures (sim_a #st #o #r (absmerge ltr atr btr) (merge_a #st #o #r ltr l atr a btr b)))
 
 #set-options "--z3rlimit 10000000"
-let prop_merge2 #st #o #m ltr l atr a btr b = 
-  prop_merge21 #st #o #m ltr l atr a btr b;
-  prop_merge22 #st #o #m ltr l atr a btr b
+let prop_merge_a #st #o #r #m ltr l atr a btr b = 
+  prop_merge21 #st #o #r #m ltr l atr a btr b;
+  prop_merge22 #st #o #r #m ltr l atr a btr b;
+  let m1 = get_lst (merge_a #st #o #r ltr l atr a btr b) in
+  prop_merge1 #st #o #r #m ltr l atr a btr b m1
 
-val prop_merge31 : #st:eqtype -> #o:eqtype -> #m:(mrdt st o) -> {|alpha_map st o m|}
-          -> ltr:ae (op o)
-          -> l:s st
-          -> atr:ae (op o)
-          -> a:s st
-          -> btr:ae (op o)
-          -> b:s st
-          -> Lemma (requires (forall e. mem e ltr.l ==> not (mem_id (get_id e) atr.l)) /\
-                            (forall e. mem e atr.l ==> not (mem_id (get_id e) btr.l)) /\
-                            (forall e. mem e ltr.l ==> not (mem_id (get_id e) btr.l)) /\
-                            (sim_a ltr l /\ sim_a (union ltr atr) a /\ sim_a (union ltr btr) b) /\
-                             pre_cond_merge1_a #st #o l a b /\
-                            (forall ch. mem_key_s ch a \/ mem_key_s ch b ==> 
-                            (pre_cond_merge #st #o (project ch ltr) (get_val_s #st #o ch l)
-                                                   (project ch atr) (get_val_s #st #o ch a)
-                                                   (project ch btr) (get_val_s #st #o ch b)) /\
-                            (forall e. mem e (project ch ltr).l ==> not (mem_id (get_id e) (project ch atr).l)) /\
-                            (forall e. mem e (project ch atr).l ==> not (mem_id (get_id e) (project ch btr).l)) /\
-                            (forall e. mem e (project ch ltr).l ==> not (mem_id (get_id e) (project ch btr).l)) /\
-                            (sim #st #o (project ch ltr) (get_val_s #st #o ch l) /\ sim #st #o (union (project ch ltr) (project ch atr)) (get_val_s #st #o ch a) /\ sim #st #o (union (project ch ltr) (project ch btr)) (get_val_s #st #o ch b))) /\ (forall ch. mem_key_s ch (merge_a ltr l atr a btr b) <==> mem_key ch (absmerge ltr atr btr).l))
-                    (ensures (forall e. mem e (absmerge ltr atr btr).l ==> 
-                             (exists e1. mem e1 (merge_a ltr l atr a btr b) /\ get_key e = get_key_s e1)))
-
-#set-options "--z3rlimit 10000000"
-let prop_merge31 #st #o #m ltr l atr a btr b = 
-  lemma2 #st #o #m (merge_a ltr l atr a btr b);
-  lemma6 ltr atr; lemma6 ltr btr;
-  lemma61 ltr atr btr
-
-val prop_merge_a : #st:eqtype -> #o:eqtype -> #m:(mrdt st o) -> {|alpha_map st o m|}
-          -> ltr:ae (op o)
-          -> l:s st
-          -> atr:ae (op o)
-          -> a:s st
-          -> btr:ae (op o)
-          -> b:s st
-          -> Lemma (requires (forall e. mem e ltr.l ==> not (mem_id (get_id e) atr.l)) /\
-                            (forall e. mem e atr.l ==> not (mem_id (get_id e) btr.l)) /\
-                            (forall e. mem e ltr.l ==> not (mem_id (get_id e) btr.l)) /\
-                            (sim_a ltr l /\ sim_a (union ltr atr) a /\ sim_a (union ltr btr) b) /\
-                             pre_cond_merge1_a #st #o l a b /\
-                            (forall ch. mem_key_s ch a \/ mem_key_s ch b ==> 
-                            (pre_cond_merge #st #o (project ch ltr) (get_val_s #st #o ch l)
-                                                   (project ch atr) (get_val_s #st #o ch a)
-                                                   (project ch btr) (get_val_s #st #o ch b)) /\
-                            (forall e. mem e (project ch ltr).l ==> not (mem_id (get_id e) (project ch atr).l)) /\
-                            (forall e. mem e (project ch atr).l ==> not (mem_id (get_id e) (project ch btr).l)) /\
-                            (forall e. mem e (project ch ltr).l ==> not (mem_id (get_id e) (project ch btr).l)) /\
-                            (sim #st #o (project ch ltr) (get_val_s #st #o ch l) /\ sim #st #o (union (project ch ltr) (project ch atr)) (get_val_s #st #o ch a) /\ sim #st #o (union (project ch ltr) (project ch btr)) (get_val_s #st #o ch b))))
-                    (ensures (sim_a (absmerge ltr atr btr) (merge_a ltr l atr a btr b)))
-
-#set-options "--z3rlimit 10000000"
-let prop_merge_a #st #o #m ltr l atr a btr b = 
-  prop_merge2 #st #o #m ltr l atr a btr b;
-  prop_merge31 #st #o #m ltr l atr a btr b;
-  let m1 = get_lst (merge_a ltr l atr a btr b) in
-  prop_merge1 #st #o #m ltr l atr a btr b m1
-
+val prop_spec : #st:eqtype -> #o:eqtype -> #r:eqtype -> {|mrdt st o r|}
+              -> tr:ae (op o)
+              -> st1:(s st)
+              -> op:(nat * (op o))
+              -> Lemma (requires (sim_a #st #o #r tr st1) /\ (not (mem_id (get_id op) tr.l)) /\
+                                (forall e. mem e tr.l ==> get_id e < get_id op) /\ get_id op > 0)
+                      (ensures true (*get_rval (app_op st op)) = spec_a op tr*))
+#set-options "--z3rlimit 1000000"
+let prop_spec tr st op = ()
 
