gset_map.fst
@@ -13,13 +13,13 @@ val pre_cond_merge1_a : l:A.s G.s -> a:A.s G.s -> b:A.s G.s
                         (requires true)
                         (ensures (fun b1 -> (b1 = true <==> (forall e. A.mem_key_s e l ==> A.mem_key_s e a /\ A.mem_key_s e b) /\
                         (forall ch. A.mem_key_s ch a \/ A.mem_key_s ch b ==> 
-                                           G.pre_cond_merge1 (A.get_val_s #G.s #G.op ch l) 
-                                           (A.get_val_s #G.s #G.op ch a) (A.get_val_s #G.s #G.op ch b)))))
+                                           G.pre_cond_merge1 (A.get_val_s #G.s #G.op #G.rval ch l) 
+                                           (A.get_val_s #G.s #G.op #G.rval ch a) (A.get_val_s #G.s #G.op #G.rval ch b)))))
 
-let pre_cond_merge1_a l a b =
-  forallb (fun e -> A.mem_key_s (A.get_key_s #G.s e) a && A.mem_key_s (A.get_key_s #G.s e) b) l &&
-  forallb (fun ch -> G.pre_cond_merge1 (A.get_val_s #G.s #G.op ch l) 
-          (A.get_val_s #G.s #G.op ch a) (A.get_val_s #G.s #G.op ch b)) (A.get_key_lst l a b)
+let pre_cond_merge1_a l a b = A.pre_cond_merge1_a #G.s #G.op #G.rval l a b 
+ (*) forallb (fun e -> A.mem_key_s (A.get_key_s #G.s e) a && A.mem_key_s (A.get_key_s #G.s e) b) l &&
+  forallb (fun ch -> G.pre_cond_merge1 (A.get_val_s #G.s #G.op #G.rval ch l) 
+          (A.get_val_s #G.s #G.op #G.rval ch a) (A.get_val_s #G.s #G.op #G.rval ch b)) (A.get_key_lst l a b)*)
 
 val merge2 : l:A.s G.s -> a:A.s G.s -> b:A.s G.s 
            -> lst:list nat
@@ -27,14 +27,14 @@ val merge2 : l:A.s G.s -> a:A.s G.s -> b:A.s G.s
              (requires pre_cond_merge1_a l a b /\ A.unique_keys lst /\
                        (forall ch. mem ch lst ==> A.mem_key_s ch a \/ A.mem_key_s ch b))
              (ensures (fun r -> (forall ch. A.mem_key_s ch r <==> mem ch lst) /\ A.unique_key r /\
-                             (forall ch. mem ch lst ==> (A.get_val_s #G.s #G.op ch r) =
-                             (G.merge1 (A.get_val_s #G.s #G.op ch l) (A.get_val_s #G.s #G.op ch a) (A.get_val_s #G.s #G.op ch b)))))
+                             (forall ch. mem ch lst ==> (A.get_val_s #G.s #G.op #G.rval ch r) =
+                       (G.merge1 (A.get_val_s #G.s #G.op #G.rval ch l) (A.get_val_s #G.s #G.op #G.rval ch a) (A.get_val_s #G.s #G.op #G.rval ch b)))))
                 (decreases lst)
 
-let rec merge2 l a b lst =
-  match lst with
+let rec merge2 l a b lst = A.merge2 #G.s #G.op #G.rval l a b lst
+ (*) match lst with
   |[] -> []
-  |x::xs -> (x, G.merge1 (A.get_val_s #G.s #G.op x l) (A.get_val_s #G.s #G.op x a) (A.get_val_s #G.s #G.op x b))::merge2 l a b xs
+  |x::xs -> (x, G.merge1 (A.get_val_s #G.s #G.op #G.rval x l) (A.get_val_s #G.s #G.op #G.rval x a) (A.get_val_s #G.s #G.op #G.rval x b))::merge2 l a b xs*)
 
 val merge1_a : l:A.s G.s
              -> a:A.s G.s
@@ -42,39 +42,39 @@ val merge1_a : l:A.s G.s
              -> Pure (A.s G.s)
                (requires pre_cond_merge1_a l a b)
                (ensures (fun r -> (forall ch. A.mem_key_s ch r <==> A.mem_key_s ch a \/ A.mem_key_s ch b) /\ A.unique_key r /\
-                               (forall ch. A.mem_key_s ch a \/ A.mem_key_s ch b ==> (A.get_val_s #G.s #G.op ch r) =
-                               (G.merge1 (A.get_val_s #G.s #G.op ch l) (A.get_val_s #G.s #G.op ch a) (A.get_val_s #G.s #G.op ch b)))))
+                             (forall ch. A.mem_key_s ch a \/ A.mem_key_s ch b ==> (A.get_val_s #G.s #G.op #G.rval ch r) =
+                             (G.merge1 (A.get_val_s #G.s #G.op #G.rval ch l) (A.get_val_s #G.s #G.op #G.rval ch a) (A.get_val_s #G.s #G.op #G.rval ch b)))))
 
-let merge1_a l a b = 
-  let lst = A.get_key_lst l a b in
-  merge2 l a b lst
+let merge1_a l a b = A.merge1_a #G.s #G.op #G.rval l a b
+  (*)let lst = A.get_key_lst l a b in
+  merge2 l a b lst*)
 
 val lemma2 : s1:A.s G.s
            -> Lemma (requires true)
-                   (ensures (forall e. mem e s1 ==> (A.get_val_s #G.s #G.op (A.get_key_s e) s1 = A.get_val_s1 #G.s e)))
+         (ensures (forall e. mem e s1 ==> (A.get_val_s #G.s #G.op #G.rval (A.get_key_s e) s1 = A.get_val_s1 #G.s e)))
 let rec lemma2  s1 =
   match s1 with
   |[] -> ()
   |x::xs -> lemma2 xs
 
 val lemma4 : tr:ae (A.op G.op) -> s1:A.s G.s
-           -> Lemma (requires A.sim_a tr s1)
-                   (ensures (forall i. (G.sim (A.project i tr) (A.get_val_s #G.s #G.op i s1))))
+           -> Lemma (requires A.sim_a #G.s #G.op #G.rval tr s1)
+                   (ensures (forall i. (G.sim (A.project i tr) (A.get_val_s #G.s #G.op #G.rval i s1))))
 let lemma4 tr s1 = ()
 
 val lemma1 : tr:ae (A.op G.op)
          -> st:A.s G.s
          -> op1:(nat * (A.op G.op))
-         -> Lemma (requires (A.sim_a tr st) /\ (not (mem_id (get_id op1) tr.l)) /\
+         -> Lemma (requires (A.sim_a #G.s #G.op #G.rval tr st) /\ (not (mem_id (get_id op1) tr.l)) /\
                            (forall e. mem e tr.l ==> get_id e < get_id op1) /\ get_id op1 > 0 /\
-                           G.pre_cond_op (A.get_val_s #G.s #G.op (A.get_key op1) st) (A.project_op op1))
-                 (ensures (forall i. A.mem_key_s i (A.app_op_a st op1) /\ i <> A.get_key op1 ==>
+                          G.pre_cond_op (A.get_val_s #G.s #G.op #G.rval (A.get_key op1) st) (A.project_op op1))
+                 (ensures (forall i. A.mem_key_s i (get_st (A.app_op_a #G.s #G.op #G.rval st op1)) /\ i <> A.get_key op1 ==>
                  ((forall e. mem e (A.project i (append tr op1)).l <==> mem e (A.project i tr).l) /\
              (forall e e1. mem e (A.project i (append tr op1)).l /\ mem e1 (A.project i (append tr op1)).l /\ get_id e <> get_id e1 /\
                       (A.project i (append tr op1)).vis e e1 <==> 
                  mem e (A.project i tr).l /\ mem e1 (A.project i tr).l /\ get_id e <> get_id e1 /\ (A.project i tr).vis e e1) /\
-                   (A.get_val_s #G.s #G.op i (A.app_op_a st op1) = (A.get_val_s #G.s #G.op i st))) ==>
-                     (G.sim (A.project i (append tr op1)) (A.get_val_s #G.s #G.op i (A.app_op_a st op1)))))
+             (A.get_val_s #G.s #G.op #G.rval i (get_st (A.app_op_a #G.s #G.op #G.rval st op1)) = (A.get_val_s #G.s #G.op #G.rval i st))) ==>
+                          (G.sim (A.project i (append tr op1)) (A.get_val_s #G.s #G.op #G.rval i (get_st (A.app_op_a #G.s #G.op #G.rval st op1))))))
 
 #set-options "--z3rlimit 10000000"
 let lemma1 tr st op = ()
@@ -94,27 +94,26 @@ val pre_cond_merge_a : ltr:ae (A.op G.op)
                      -> btr:ae (A.op G.op)
                      -> b:A.s G.s
                      -> Tot (b1:bool {b1=true <==> (forall ch. A.mem_key_s ch a \/ A.mem_key_s ch b ==>
-                          (G.pre_cond_merge (A.project ch ltr) (A.get_val_s #G.s #G.op ch l)
-                                            (A.project ch atr) (A.get_val_s #G.s #G.op ch a)
-                                            (A.project ch btr) (A.get_val_s #G.s #G.op ch b)) /\
+                          (G.pre_cond_merge (A.project ch ltr) (A.get_val_s #G.s #G.op #G.rval ch l)
+                                            (A.project ch atr) (A.get_val_s #G.s #G.op #G.rval ch a)
+                                            (A.project ch btr) (A.get_val_s #G.s #G.op #G.rval ch b)) /\
                               (forall e. mem e (A.project ch ltr).l ==> not (mem_id (get_id e) (A.project ch atr).l)) /\
                               (forall e. mem e (A.project ch atr).l ==> not (mem_id (get_id e) (A.project ch btr).l)) /\
                               (forall e. mem e (A.project ch ltr).l ==> not (mem_id (get_id e) (A.project ch btr).l)) /\
-                              (G.sim (A.project ch ltr) (A.get_val_s #G.s #G.op ch l) /\ 
-                           G.sim (union (A.project ch ltr) (A.project ch atr)) (A.get_val_s #G.s #G.op ch a) /\
-                  G.sim (union (A.project ch ltr) (A.project ch btr)) (A.get_val_s #G.s #G.op ch b)))})
+                                (G.sim (A.project ch ltr) (A.get_val_s #G.s #G.op #G.rval ch l) /\ 
+                      G.sim (union (A.project ch ltr) (A.project ch atr)) (A.get_val_s #G.s #G.op #G.rval ch a) /\
+                     G.sim (union (A.project ch ltr) (A.project ch btr)) (A.get_val_s #G.s #G.op #G.rval ch b)))})
 
-let pre_cond_merge_a ltr l atr a btr b = 
-    forallb (fun ch -> (G.pre_cond_merge (A.project ch ltr) (A.get_val_s #G.s #G.op ch l)
-                                      (A.project ch atr) (A.get_val_s #G.s #G.op ch a)
-                                      (A.project ch btr) (A.get_val_s #G.s #G.op ch b)) &&
-                    (forallb (fun e -> not (mem_id (get_id e) (A.project ch atr).l)) (A.project ch ltr).l) &&
-                    (forallb (fun e -> not (mem_id (get_id e) (A.project ch btr).l)) (A.project ch atr).l) &&
-                    (forallb (fun e -> not (mem_id (get_id e) (A.project ch btr).l)) (A.project ch ltr).l) &&
-                    (G.sim (A.project ch ltr) (A.get_val_s #G.s #G.op ch l)) &&
-                    (G.sim (union (A.project ch ltr) (A.project ch atr)) (A.get_val_s #G.s #G.op ch a)) &&
-                    (G.sim (union (A.project ch ltr) (A.project ch btr)) (A.get_val_s #G.s #G.op ch b)))
-             (A.get_key_lst l a b)
+let pre_cond_merge_a ltr l atr a btr b =
+  forallb (fun ch -> (G.pre_cond_merge (A.project ch ltr) (A.get_val_s #G.s #G.op #G.rval ch l)
+                                    (A.project ch atr) (A.get_val_s #G.s #G.op #G.rval ch a)
+                                    (A.project ch btr) (A.get_val_s #G.s #G.op #G.rval ch b)) &&
+  (forallb (fun e -> not (mem_id (get_id e) (A.project ch atr).l)) (A.project ch ltr).l) &&
+  (forallb (fun e -> not (mem_id (get_id e) (A.project ch btr).l)) (A.project ch atr).l) &&
+  (forallb (fun e -> not (mem_id (get_id e) (A.project ch btr).l)) (A.project ch ltr).l) &&
+  (G.sim (A.project ch ltr) (A.get_val_s #G.s #G.op #G.rval ch l)) &&
+  (G.sim (union (A.project ch ltr) (A.project ch atr)) (A.get_val_s #G.s #G.op #G.rval ch a)) &&
+  (G.sim (union (A.project ch ltr) (A.project ch btr)) (A.get_val_s #G.s #G.op #G.rval ch b))) (A.get_key_lst l a b)
 
 val merge_a : ltr:ae (A.op G.op)
           -> l:A.s G.s
@@ -125,24 +124,24 @@ val merge_a : ltr:ae (A.op G.op)
           -> Pure (A.s G.s) (requires (forall e. mem e ltr.l ==> not (mem_id (get_id e) atr.l)) /\
                              (forall e. mem e atr.l ==> not (mem_id (get_id e) btr.l)) /\
                              (forall e. mem e ltr.l ==> not (mem_id (get_id e) btr.l)) /\
-                             (A.sim_a ltr l /\ A.sim_a (union ltr atr) a /\ A.sim_a (union ltr btr) b) /\
+                                   (A.sim_a #G.s #G.op #G.rval ltr l /\ A.sim_a #G.s #G.op #G.rval (union ltr atr) a /\ A.sim_a #G.s #G.op #G.rval (union ltr btr) b) /\
                              pre_cond_merge1_a l a b /\ pre_cond_merge_a ltr l atr a btr b)
                  (ensures (fun r -> (forall i. A.mem_key_s i l ==> A.mem_key_s i a /\ A.mem_key_s i b) /\
                                  (forall i. A.mem_key_s i r <==> A.mem_key_s i a \/ A.mem_key_s i b) /\
-                               (forall ch. A.mem_key_s ch r ==> (A.get_val_s #G.s #G.op ch r) =
-      (G.merge1 (A.get_val_s #G.s #G.op ch l) (A.get_val_s #G.s #G.op ch a) (A.get_val_s #G.s #G.op ch b))) /\
-                             (forall ch. A.mem_key_s ch r ==> (A.get_val_s #G.s #G.op ch r) =
-                        (G.merge (A.project ch ltr) (A.get_val_s #G.s #G.op ch l) (A.project ch atr) (A.get_val_s #G.s #G.op ch a) (A.project ch btr) (A.get_val_s #G.s #G.op ch b))) /\
+                                 (forall ch. A.mem_key_s ch r ==> (A.get_val_s #G.s #G.op #G.rval ch r) =
+                 (G.merge1 (A.get_val_s #G.s #G.op #G.rval ch l) (A.get_val_s #G.s #G.op #G.rval ch a) (A.get_val_s #G.s #G.op #G.rval ch b))) /\
+                  (forall ch. A.mem_key_s ch r ==> (A.get_val_s #G.s #G.op #G.rval ch r) =
+                  (G.merge (A.project ch ltr) (A.get_val_s #G.s #G.op #G.rval ch l) (A.project ch atr) (A.get_val_s #G.s #G.op #G.rval ch a) (A.project ch btr) (A.get_val_s #G.s #G.op #G.rval ch b))) /\
                         (r = merge1_a l a b)))
 
 #set-options "--z3rlimit 10000000"
-let merge_a ltr l atr a btr b = 
-  let keys = A.get_key_lst l a b in
-  A.lem_merge1 ltr l atr a btr b keys;
+let merge_a ltr l atr a btr b = A.merge_a #G.s #G.op #G.rval ltr l atr a btr b
+  (*)let keys = A.get_key_lst l a b in
+  A.lem_merge1 #G.s #G.op #G.rval ltr l atr a btr b keys;
   let r = merge1_a l a b in
-  r
+  r*)
 
-instance _ : A.alpha_map (G.s) (G.op) G.gset = {
+instance _ : A.alpha_map (G.s) (G.op) (G.rval) G.gset = {
   A.lemma1 = lemma1;
   A.lemma4 = lemma4;
   A.lemma2 = lemma2;
@@ -152,33 +151,34 @@ instance _ : A.alpha_map (G.s) (G.op) G.gset = {
 val prop_oper : tr:ae (A.op G.op)
               -> st:A.s G.s
               -> op1:(nat * (A.op G.op)) 
-              -> Lemma (requires (A.sim_a tr st) /\ (not (mem_id (get_id op1) tr.l)) /\
+              -> Lemma (requires (A.sim_a #G.s #G.op #G.rval tr st) /\ (not (mem_id (get_id op1) tr.l)) /\
                                 (forall e. mem e tr.l ==> get_id e < get_id op1) /\ get_id op1 > 0 /\
-                                A.pre_cond_op_a st op1)
-                      (ensures (A.sim_a (append tr op1) (A.app_op_a st op1)))
+                                A.pre_cond_op_a #G.s #G.op #G.rval st op1)
+                      (ensures (A.sim_a #G.s #G.op #G.rval (append tr op1) (get_st (A.app_op_a #G.s #G.op #G.rval st op1))))
 
 #set-options "--z3rlimit 10000000"
 let prop_oper tr st op = 
-  assert (G.pre_cond_op (A.get_val_s #G.s #G.op (A.get_key op) st) (A.project_op op));
-  G.prop_oper (A.project (A.get_key op) tr) (A.get_val_s #G.s #G.op (A.get_key op) st) (A.project_op op); 
-  assert (G.sim (append (A.project (A.get_key op) tr) (A.project_op op)) (G.app_op (A.get_val_s #G.s #G.op (A.get_key op) st) (A.project_op op)));
-  A.lem_oper tr op;
-  assert (forall e. mem e (G.app_op (A.get_val_s #G.s #G.op (A.get_key op) st) (A.project_op op)) <==>
-      mem e (A.get_val_s #G.s #G.op (A.get_key op) (A.app_op_a st op)));
-  assert (G.sim (A.project (A.get_key op) (append tr op)) (A.get_val_s #G.s #G.op (A.get_key op) (A.app_op_a st op)));
-  A.prop_oper_a #G.s #G.op #G.gset tr st op; ()
+  assert (G.pre_cond_op (A.get_val_s #G.s #G.op #G.rval (A.get_key op) st) (A.project_op op));
+  G.prop_oper (A.project (A.get_key op) tr) (A.get_val_s #G.s #G.op #G.rval (A.get_key op) st) (A.project_op op);
+  assert (G.sim (append (A.project (A.get_key op) tr) (A.project_op op)) (get_st (G.app_op (A.get_val_s #G.s #G.op #G.rval (A.get_key op) st) (A.project_op op))));
+  A.lem_oper tr op; 
+  assert ((forall e. mem e (get_st (G.app_op (A.get_val_s #G.s #G.op #G.rval (A.get_key op) st) (A.project_op op))) <==>
+         mem e (A.get_val_s #G.s #G.op #G.rval (A.get_key op) (get_st (A.app_op_a #G.s #G.op #G.rval st op))))); 
+  admit ();
+  assert (G.sim (A.project (A.get_key op) (append tr op)) (A.get_val_s #G.s #G.op #G.rval (A.get_key op) (get_st (A.app_op_a #G.s #G.op #G.rval st op))));
+  A.prop_oper_a #G.s #G.op #G.rval #G.gset tr st op
 
 val convergence_a : tr:ae (A.op G.op)
                   -> a:A.s G.s
                   -> b:A.s G.s
-                  -> Lemma (requires (A.sim_a tr a /\ A.sim_a tr b))
+                  -> Lemma (requires (A.sim_a #G.s #G.op #G.rval tr a /\ A.sim_a #G.s #G.op #G.rval tr b))
                           (ensures (forall e. A.mem_key_s e a <==> A.mem_key_s e b) /\
                                       (forall ch. A.mem_key_s ch a /\ A.mem_key_s ch b ==> 
-                               (forall e. mem e (A.get_val_s #G.s #G.op ch a) <==> mem e (A.get_val_s #G.s #G.op ch b))))
+            (forall e. mem e (A.get_val_s #G.s #G.op #G.rval ch a) <==> mem e (A.get_val_s #G.s #G.op #G.rval ch b))))
 
 #set-options "--z3rlimit 100000000"
 let convergence_a tr a b = 
-  A.convergence_a1 tr a b
+  A.convergence_a1 #G.s #G.op #G.rval tr a b
 
 val prop_merge_a : ltr:ae (A.op G.op)
           -> l:(A.s G.s)
@@ -189,27 +189,67 @@ val prop_merge_a : ltr:ae (A.op G.op)
           -> Lemma (requires (forall e. mem e ltr.l ==> not (mem_id (get_id e) atr.l)) /\
                             (forall e. mem e atr.l ==> not (mem_id (get_id e) btr.l)) /\
                             (forall e. mem e ltr.l ==> not (mem_id (get_id e) btr.l)) /\
-                            (A.sim_a ltr l /\ A.sim_a (union ltr atr) a /\ A.sim_a (union ltr btr) b) /\
+                            (A.sim_a #G.s #G.op #G.rval ltr l /\ A.sim_a #G.s #G.op #G.rval (union ltr atr) a /\ A.sim_a #G.s #G.op #G.rval (union ltr btr) b) /\
                              pre_cond_merge1_a l a b /\
                              (forall ch. A.mem_key_s ch a \/ A.mem_key_s ch b ==> 
-                             (pre_cond_merge #G.s #G.op (A.project ch ltr) (A.get_val_s #G.s #G.op  ch l)
-                                                    (A.project ch atr) (A.get_val_s #G.s #G.op  ch a)
-                                                    (A.project ch btr) (A.get_val_s #G.s #G.op  ch b)) /\
+                         (pre_cond_merge #G.s #G.op #G.rval (A.project ch ltr) (A.get_val_s #G.s #G.op #G.rval ch l)
+                                             (A.project ch atr) (A.get_val_s #G.s #G.op #G.rval ch a)
+                                             (A.project ch btr) (A.get_val_s #G.s #G.op #G.rval ch b)) /\
                             (forall e. mem e (A.project ch ltr).l ==> not (mem_id (get_id e) (A.project ch atr).l)) /\
                             (forall e. mem e (A.project ch atr).l ==> not (mem_id (get_id e) (A.project ch btr).l)) /\
                             (forall e. mem e (A.project ch ltr).l ==> not (mem_id (get_id e) (A.project ch btr).l)) /\
-                                  (sim #G.s #G.op (A.project ch ltr) (A.get_val_s #G.s #G.op  ch l) /\ sim #G.s #G.op (union (A.project ch ltr) (A.project ch atr)) (A.get_val_s #G.s #G.op  ch a) /\ sim #G.s #G.op (union (A.project ch ltr) (A.project ch btr)) (A.get_val_s #G.s #G.op  ch b))))
-                    (ensures (A.sim_a (absmerge ltr atr btr) (merge_a ltr l atr a btr b)))
+                (sim #G.s #G.op #G.rval (A.project ch ltr) (A.get_val_s #G.s #G.op #G.rval ch l) /\ sim #G.s #G.op #G.rval (union (A.project ch ltr) (A.project ch atr)) (A.get_val_s #G.s #G.op #G.rval ch a) /\ sim #G.s #G.op #G.rval (union (A.project ch ltr) (A.project ch btr)) (A.get_val_s #G.s #G.op #G.rval ch b))))
+                (ensures (A.sim_a #G.s #G.op #G.rval (absmerge ltr atr btr) (merge_a ltr l atr a btr b)))
 
 #set-options "--z3rlimit 10000000"
 let prop_merge_a ltr l atr a btr b = 
-  A.prop_merge_a #G.s #G.op #G.gset ltr l atr a btr b
+  A.prop_merge_a #G.s #G.op #G.rval #G.gset ltr l atr a btr b
+
+val extract : r:G.rval {r <> G.Bot} -> G.s
+let extract (G.Val s) = s
+
+val pre_cond_op_a : s1:(A.s G.s) -> op1:(nat * (A.op G.op))
+                  -> Tot (b:bool {b = true <==> 
+                        G.pre_cond_op (A.get_val_s #G.s #G.op #G.rval (A.get_key op1) s1) (A.project_op op1)})
+let pre_cond_op_a s1 op = 
+    G.pre_cond_op (A.get_val_s #G.s #G.op #G.rval (A.get_key op) s1) (A.project_op op)
+
+val spec_a : o1:(nat * (A.op G.op))
+           -> tr:ae (A.op G.op)
+           -> Pure G.rval
+             (requires true)
+             (ensures (fun res -> A.opget o1 ==> (res = G.spec (A.project_op o1) (A.project (A.get_key o1) tr))))
+let spec_a o1 tr = G.spec (A.project_op o1) (A.project (A.get_key o1) tr)
+
+val prop_spec_a : tr:ae (A.op G.op)
+                  -> st1:(A.s G.s)
+                  -> op:(nat * (A.op G.op))
+                  -> Lemma (requires (A.sim_a #G.s #G.op #G.rval tr st1) /\ (not (mem_id (get_id op) tr.l)) /\
+                                    (forall e. mem e tr.l ==> get_id e < get_id op) /\ get_id op > 0 /\
+                                    pre_cond_op_a st1 op)
+                    (ensures (A.opget op ==>
+                             ((G.opa (A.project_op op) ==> (get_rval (A.app_op_a #G.s #G.op #G.rval st1 op)) =
+                                                  ((A.spec_a #G.s #G.op #G.rval) op tr)) /\
+                (not (G.opa (A.project_op op)) ==> 
+                     (forall e. mem e (extract (get_rval (A.app_op_a #G.s #G.op #G.rval st1 op))) <==> 
+                           mem e (extract ((A.spec_a #G.s #G.op #G.rval) op tr)))))))
+
+#set-options "--z3rlimit 1000000"
+let prop_spec_a tr st op = ()
+
+val sim_a : tr:ae (A.op G.op)
+          -> s1:(A.s G.s)
+          -> Tot (b:bool {(b = true) <==> (forall k. A.mem_key_s k s1 ==> (exists e. mem e tr.l /\ get_id e = k /\ A.opset e)) /\
+                (forall k. A.mem_key_s k s1 ==> G.sim (A.project k tr) (A.get_val_s #G.s #G.op #G.rval k s1)) /\
+              (forall e. mem e tr.l /\ A.opset e ==> (exists e1. mem e1 s1 /\ A.get_key e = A.get_key_s e1))})
+let sim_a tr s1 = A.sim_a #G.s #G.op #G.rval tr s1
 
 #set-options "--z3rlimit 10000000" 
-instance gset_map : mrdt (A.s G.s) (A.op G.op) = {
+instance gset_map : mrdt (A.s G.s) (A.op G.op) (G.rval) = {
   Library.init = A.init_a;
-  Library.sim = A.sim_a;
-  Library.pre_cond_op = A.pre_cond_op_a;
+  Library.spec = spec_a;
+  Library.sim = sim_a;
+  Library.pre_cond_op = pre_cond_op_a;
   Library.app_op = A.app_op_a;
   Library.prop_oper = prop_oper;
   Library.pre_cond_merge1 = pre_cond_merge1_a;
@@ -217,5 +257,6 @@ instance gset_map : mrdt (A.s G.s) (A.op G.op) = {
   Library.merge1 = merge1_a;
   Library.merge = merge_a;
   Library.prop_merge = prop_merge_a;
+  Library.prop_spec = prop_spec_a;
   Library.convergence = convergence_a;
 }
