ictr.fst
@@ -5,23 +5,36 @@ open Library
 
 type s = nat
 
-type op = |Add 
+type rval = |Val : s -> rval
+            |Bot
+
+type op = |Add
+          |Rd
 
 let init = 0
 
 let pre_cond_op s1 op = true
 
-val app_op : s1:s -> op:(nat * op) -> Tot (s2:s {s2 = s1 + 1})
+val app_op : s1:s -> op:(nat * op) -> Tot (s2:(s * rval) {get_op op = Add ==> s2 = (s1 + 1, Bot) /\
+                                                      get_op op = Rd ==> s2 = (s1, Val s1)})
 let app_op s op1 =
   match op1 with
-  |(_,Add) -> s + 1
+  |(_,Add) -> (s + 1, Bot)
+  |(_,Rd) -> (s, Val s)
 
 val sum : l:(list (nat * op))
-        -> Tot (n:nat {n = (List.Tot.length l)}) (decreases %[l])
+        -> Tot (n:nat {n = (List.Tot.length (filter (fun e -> get_op e = Add) l))}) (decreases %[l])
 let rec sum l =
   match l with
   |[] -> 0
   |(_, Add)::xs -> sum xs + 1
+  |(_, Rd)::xs -> sum xs
+
+val spec : o:(nat * op) -> tr:ae op -> r:rval
+let spec o tr =
+  match o with
+  |(_, Add) -> Bot
+  |(_, Rd) -> Val (sum tr.l)
 
 #set-options "--query_stats"
 val sim : tr:ae op
@@ -110,7 +123,7 @@ val prop_oper : tr:ae op
               -> op:(nat * op)
               -> Lemma (requires (sim tr st) /\ (not (mem_id (get_id op) tr.l)) /\
                                 (forall e. mem e tr.l ==> get_id e < get_id op) /\ get_id op > 0)
-                      (ensures (sim (append tr op) (app_op st op)))
+                      (ensures (sim (append tr op) (get_st (app_op st op))))
 let prop_oper tr st op = ()
 
 val convergence : tr:ae op
@@ -120,8 +133,17 @@ val convergence : tr:ae op
                         (ensures a = b)
 let convergence tr a b = ()
 
-instance _ : mrdt s op = {
+val prop_spec : tr:ae op
+              -> st:s
+              -> op:(nat * op)
+              -> Lemma (requires (sim tr st) /\ (not (mem_id (get_id op) tr.l)) /\
+                                (forall e. mem e tr.l ==> get_id e < get_id op) /\ get_id op > 0)
+                      (ensures (get_rval (app_op st op) = spec op tr))
+let prop_spec tr st op = ()
+
+instance ictr : mrdt s op rval = {
   Library.init = init;
+  Library.spec = spec;
   Library.sim = sim;
   Library.pre_cond_op = pre_cond_op;
   Library.app_op = app_op;
@@ -131,6 +153,7 @@ instance _ : mrdt s op = {
   Library.merge1 = merge1;
   Library.merge = merge;
   Library.prop_merge = prop_merge;
+  Library.prop_spec = prop_spec;
   Library.convergence = convergence
 }
 
