lww.fst
@@ -5,7 +5,23 @@ open Library
 
 type s = (nat (*timestamp*) * nat (*value*))
 
-type op = nat (*value*)
+type rval = |Val : nat -> rval
+            |Bot
+
+type op = |Write : nat -> op
+          |Rd
+
+val opw : (nat * op) -> bool
+let opw o =
+  match o with
+  |(_, Write _) -> true
+  |(_, Rd) -> false
+
+val opr : (nat * op) -> bool
+let opr o = not (opw o)
+
+val get_val : o:(nat * op){opw o} -> nat
+let get_val (_, Write n) = n
 
 val get_id_s : s -> nat
 let get_id_s (t, v) = t
@@ -14,16 +30,21 @@ let get_ele_s (t, v) = v
 
 let pre_cond_op s1 op = true
 
-val app_op : s1:s -> op:(nat * op) -> Tot (s2:s {s2 = ((get_id op), (get_op op))})
-let app_op (t, v) (t1, v1) = (t1, v1)
+val app_op : s1:s -> op:(nat * op) -> Tot (s2:(s * rval) {(opw op ==> s2 = (((get_id op), (get_val op)), Bot)) /\
+                                                      (opr op ==> s2 = (s1, Val (get_ele_s s1)))})
+let app_op s1 o =
+  match o with
+  |(t, Write n) -> ((t, n), Bot)
+  |(_, Rd) -> (s1, Val (get_ele_s s1))
 
 val mem_ele : v:nat
             -> l:list (nat * op)
-            -> Tot (b:bool{(exists id. mem (id, v) l) <==> b=true})
+            -> Tot (b:bool{(exists id. mem (id, Write v) l) <==> b=true})
 let rec mem_ele n l =
   match l with
   |[] -> false
-  |(_, v)::xs -> (n = v) || mem_ele n xs
+  |(_, Write v)::xs -> (n = v) || mem_ele n xs
+  |(_, Rd)::xs -> mem_ele n xs
 
 val init : s
 let init = (0,0)
@@ -32,23 +53,31 @@ val gt : l:list (nat * op)
        -> init1:s
        -> Pure s
          (requires true)
-         (ensures (fun r -> (mem ((get_id_s r), (get_ele_s r)) l \/ r = init1) /\
-                         (forall e. mem e l ==> get_id_s r >= get_id e) /\ (get_id_s r >= get_id_s init1)))
+         (ensures (fun r -> (mem ((get_id_s r), Write (get_ele_s r)) l \/ r = init1) /\
+                         (forall e. mem e l /\ opw e ==> get_id_s r >= get_id e) /\ (get_id_s r >= get_id_s init1)))
          (decreases (length l))
 #set-options "--z3rlimit 10000"
 let rec gt l init1 =
   match l with
   |[] -> init1
-  |(t, n)::xs -> if t > get_id_s init1 then (gt xs (t,n)) else (gt xs init1)
+  |(t, Write n)::xs -> if t > get_id_s init1 then (gt xs (t, n)) else (gt xs init1)
+  |(t, Rd)::xs -> gt xs init1
 
 val find : l:list (nat * op)
          -> id:nat
          -> Pure nat
-           (requires (unique_id l) /\ mem_id id l)
-           (ensures (fun v -> (mem (id, v) l) /\ mem_ele v l))
+           (requires (unique_id l) /\ mem_id id l /\ (exists v. mem (id, Write v) l))
+           (ensures (fun v -> (mem (id, Write v) l) /\ mem_ele v l))
 let rec find l id =
   match l with
-  |(id1, v)::xs -> if id = id1 then v else find xs id
+  |(id1, Write v)::xs -> if id = id1 then v else find xs id
+  |(_, Rd)::xs -> find xs id
+
+val spec : o:(nat * op) -> tr:ae op -> rval
+let spec o tr =
+    match o with
+    |(_, Write _) -> Bot
+    |(_, Rd) -> Val (snd (gt tr.l init))
 
 #set-options "--query_stats"
 val sim : tr:ae op
@@ -87,8 +116,8 @@ let merge ltr l atr a btr b =
 
 val lemma : l:list (nat * op)
           -> Lemma (requires unique_id l)
-                  (ensures (forall ele. mem_id (get_id ele) l ==> 
-                           (mem (get_id ele, (get_op ele)) l) ==> (get_op ele = find l (get_id ele))))
+                  (ensures (forall ele. mem_id (get_id ele) l /\ (exists id v. mem (id, Write v) l) ==> 
+                           (mem (get_id ele, (get_op ele)) l) ==> (get_val ele = find l (get_id ele))))
                   (decreases (length l))
 let rec lemma l = 
   match l with
@@ -112,12 +141,20 @@ let prop_merge ltr l atr a btr b =
   lemma (absmerge ltr atr btr).l;
   ()
 
+val prop_spec : tr:ae op
+              -> st:s
+              -> op:(nat * op)
+              -> Lemma (requires (sim tr st) /\ (not (mem_id (get_id op) tr.l)) /\
+                                (forall e. mem e tr.l ==> get_id e < get_id op) /\ get_id op > 0)
+                      (ensures (get_rval (app_op st op) = spec op tr))
+let prop_spec tr st op = ()
+
 val prop_oper : tr:ae op
               -> st:s
               -> op:(nat * op)
               -> Lemma (requires (sim tr st) /\ (not (mem_id (get_id op) tr.l)) /\
                                 (forall e. mem e tr.l ==> get_id e < get_id op) /\ get_id op > 0)
-                      (ensures (sim (append tr op) (app_op st op)))
+                      (ensures (sim (append tr op) (get_st (app_op st op))))
 let prop_oper tr st op = ()
 
 val convergence : tr:ae op
@@ -127,8 +164,9 @@ val convergence : tr:ae op
                         (ensures a = b)
 let convergence tr a b = ()
 
-instance _ : mrdt s op = {
+instance lww : mrdt s op rval = {
   Library.init = init;
+  Library.spec = spec;
   Library.sim = sim;
   Library.pre_cond_op = pre_cond_op;
   Library.app_op = app_op;
@@ -138,6 +176,7 @@ instance _ : mrdt s op = {
   Library.merge1 = merge1;
   Library.merge = merge;
   Library.prop_merge = prop_merge;
+  Library.prop_spec = prop_spec;
   Library.convergence = convergence
 }
 
