orset.fst
@@ -20,8 +20,17 @@ let rec unique_s l =
 
 type s = l:list (nat (*unique id*) * nat (*element*)) {unique_s l}
 
+type rval = |Val : list nat -> rval
+            |Bot
+
 val init : s
 let init = []
+
+val mem_ele_s : ele:nat -> s1:s -> Tot (b:bool {b = true <==> (exists id. mem (id,ele) s1)})
+let rec mem_ele_s ele s =
+  match s with
+  |[] -> false
+  |(_,ele1)::xs -> ele = ele1 || mem_ele_s ele xs
 
 val filter_uni : f:((nat * nat) -> bool)
                -> l:list (nat * nat) 
@@ -38,37 +47,56 @@ let rec filter_uni f l =
 type op =
   |Add : nat (*element*) -> op
   |Rem : nat (*element*) -> op
+  |Rd
 
-val get_ele : op1:(nat * op) -> Tot (ele:nat {(exists id. op1 = (id, Add ele) \/ op1 = (id, Rem ele))})
-let get_ele op =
-  match op with
-  |(_, (Add ele)) -> ele
-  |(_, (Rem ele)) -> ele
-
-val opa : op1:(nat * op) -> Tot (b:bool {b = true <==> (exists id ele. op1 = (id, Add ele))})
+val opa : op1:(nat * op) -> Tot (b:bool {b = true <==> (exists id ele. op1 = (id, Add ele)) /\ get_op op1 <> Rd})
 let opa op1 =
   match op1 with
   |(_, Add _) -> true
   |_ -> false
 
-val opr : op1:(nat * op) -> Tot (b:bool {b = true <==> (exists id ele. op1 = (id, Rem ele))})
-let opr op1 = not (opa op1)
+val opr : op1:(nat * op) -> Tot (b:bool {b = true <==> (exists id ele. op1 = (id, Rem ele)) /\ get_op op1 <> Rd})
+let opr op1 =
+  match op1 with
+  |(_, Rem _) -> true
+  |_ -> false
+
+val mem_ele : ele:nat -> l:list (nat * op) -> Tot (b:bool {b = true <==> (exists id. mem (id, (Add ele)) l) \/ (exists id. mem (id, (Rem ele)) l)})
+let rec mem_ele ele l =
+  match l with
+  |[] -> false
+  |(_, (Add ele1))::xs -> ele = ele1 || mem_ele ele xs
+  |(_, (Rem ele1))::xs -> ele = ele1 || mem_ele ele xs
+  |(_, Rd)::xs -> mem_ele ele xs
+
+val get_ele : op1:(nat * op){get_op op1 <> Rd} -> Tot (ele:nat {(exists id. op1 = (id, Add ele) \/ op1 = (id, Rem ele))})
+let get_ele op =
+  match op with
+  |(_, (Add ele)) -> ele
+  |(_, (Rem ele)) -> ele
 
 val pre_cond_op : s1:s
              -> op:(nat * op)
              -> Tot (b:bool {b=true <==> not (member_s (get_id op) s1)})
 let pre_cond_op s1 op = not (member_s (get_id op) s1)
 
+val get_set_s : s1:s -> Tot (l:list nat {(forall e. mem e l <==> mem_ele_s e s1)})
+let rec get_set_s s1 = 
+  match s1 with
+  |[] -> []
+  |(_,ele)::xs -> if mem_ele_s ele xs then get_set_s xs else ele::get_set_s xs
+
 val app_op : s1:s
            -> op:(nat * op)
-           -> Pure s
+           -> Pure (s * rval)
                  (requires pre_cond_op s1 op)
-                 (ensures (fun res -> (opa op ==> (forall e. mem e s1 \/ e = ((get_id op), (get_ele op)) <==> mem e res)) /\
-                                 (opr op ==> (forall e. mem e res <==> mem e s1 /\ snd e <> get_ele op))))
+                 (ensures (fun res -> (opa op ==> (get_rval res = Bot) /\ (forall e. mem e s1 \/ e = ((get_id op), (get_ele op)) <==> mem e (get_st res))) /\
+                                   (opr op ==> (get_rval res = Bot) /\ (forall e. mem e (get_st res) <==> mem e s1 /\ snd e <> get_ele op)) /\ (not (opa op || opr op) ==> (get_rval res = Val (get_set_s s1)) /\ (get_st res = s1))))
 let app_op s1 op1 =
   match op1 with
-  |(id, Add ele) -> (id, ele)::s1
-  |(id, Rem ele) -> filter (fun e -> snd e <> ele) s1
+  |(id, Add ele) -> ((id, ele)::s1, Bot)
+  |(id, Rem ele) -> (filter (fun e -> snd e <> ele) s1, Bot)
+  |(_, Rd) -> (s1, Val (get_set_s s1))
 
 val filter_uni1 : f:((nat * op) -> bool)
                 -> l:list (nat * op) 
@@ -80,14 +108,53 @@ let rec filter_uni1 f l =
   |[] -> ()
   |x::xs -> filter_uni1 f xs
 
-val except : #a:eqtype 
-           -> f:(a -> bool)
-           -> l:list a
-           -> Tot (l1:list a {forall e. mem e l1 <==> mem e l /\ not (f e)})
-let rec except #a f l =
+val except : f:((nat * op) -> bool)
+           -> l:list (nat * op) {unique_id l}
+           -> Tot (l1:list (nat * op) {(forall e. mem e l1 <==> mem e l /\ not (f e)) /\ unique_id l1})
+let rec except f l =
   match l with
   |[] -> []
   |hd::tl -> if not (f hd) then hd::(except f tl) else except f tl
+
+val existsb : f:((nat * op) -> bool)
+            -> l:list (nat * op)
+            -> Tot (b:bool{(exists e. mem e l /\ f e) <==> b = true})
+let rec existsb f l =
+    match l with
+    |[] -> false
+    |hd::tl -> if f hd then true else existsb f tl
+
+val get_set : tr:list (nat * op){unique_id tr} -> Tot (s1:list nat {(forall e. mem e s1 <==> mem_ele e tr)})
+let rec get_set l =
+  match l with
+  |[] -> []
+  |(_, Add x)::xs -> if mem_ele x xs then get_set xs else x::(get_set xs)
+  |(_, Rem x)::xs -> if mem_ele x xs then get_set xs else x::(get_set xs)
+  |(_, Rd)::xs -> get_set xs
+
+val extract : r:rval {exists v. r = Val v} -> list nat
+let extract (Val s) = s
+
+val forallo : f:((nat * op) -> bool)
+            -> l:list (nat * op)
+            -> Tot (b:bool{(forall e. mem e l ==> f e) <==> b = true})
+let rec forallo f l =
+  match l with
+  |[] -> true
+  |hd::tl -> if f hd then forallo f tl else false
+
+val spec : o:(nat * op) -> tr:ae op
+         -> Tot (r:rval {(get_op o = Rd ==> r <> Bot /\ (forall e. mem e (extract r) <==> (exists id. mem (id, Add e) tr.l /\
+                                    (forall r. mem r tr.l /\ id <> get_id r /\ opr r ==>
+                                              not (e = get_ele r && (tr.vis (id, Add e) r)))))) /\
+                       (opa o ==> r = Bot) /\ (opr o ==> r = Bot)})
+let spec o tr =
+  match o with
+  |(_, Add _) -> Bot
+  |(_, Rem _) -> Bot
+  |(_, Rd) -> let lsta = (filter (fun a -> opa a) tr.l) in
+  let lstr = (filter (fun r -> opr r) tr.l) in
+  let lst = except (fun a -> get_op a <> Rd && opa a && (existsb (fun r -> get_op r <> Rd && get_op a <> Rd && opa a && opr r && get_id a <> get_id r && get_ele r = get_ele a && tr.vis a r) lstr)) lsta in Val (get_set lst)
 
 #set-options "--query_stats"
 val sim : tr:ae op
@@ -98,9 +165,9 @@ val sim : tr:ae op
 let sim tr s1 =
   let lsta = (filter (fun a -> opa a) tr.l) in
   let lstr = (filter (fun r -> opr r) tr.l) in
-  let lst = except (fun a -> (existsb (fun r -> get_id a <> get_id r && get_ele r = get_ele a && tr.vis a r) lstr)) lsta in
+  let lst = except (fun a -> get_op a <> Rd && opa a &&  (existsb (fun r -> get_op r <> Rd && get_op a <> Rd && get_id a <> get_id r && get_ele r = get_ele a && tr.vis a r) lstr)) lsta in
 
-  forallb (fun e -> mem ((get_id e), (get_ele e)) s1) lst &&
+  forallo (fun e -> get_op e <> Rd && mem ((get_id e), (get_ele e)) s1) lst &&
   forallb (fun e -> mem ((fst e), Add (snd e)) lst) s1
 
 val prop_oper : tr:ae op
@@ -108,7 +175,7 @@ val prop_oper : tr:ae op
               -> op:(nat * op)
               -> Lemma (requires (sim tr st) /\ (not (mem_id (get_id op) tr.l)) /\
                                 (forall e. mem e tr.l ==> get_id e < get_id op) /\ get_id op > 0)
-                      (ensures (sim (append tr op) (app_op st op)))
+                      (ensures (sim (append tr op) (get_st (app_op st op))))
 let prop_oper tr st op = ()
 
 val convergence : tr:ae op
@@ -219,8 +286,20 @@ let prop_merge ltr l atr a btr b =
            (absmerge ltr atr btr).vis ((fst e), Add (snd e)) r))));
     ()
 
-instance _ : mrdt s op = {
+val prop_spec : tr:ae op
+              -> st:s
+              -> op:(nat * op)
+              -> Lemma (requires (sim tr st) /\ (not (mem_id (get_id op) tr.l)) /\
+                                (forall e. mem e tr.l ==> get_id e < get_id op) /\ get_id op > 0)
+                      (ensures (get_op op = Rd ==> (forall e. mem e (extract (get_rval (app_op st op))) <==>
+                                                mem e (extract (spec op tr)))) /\
+                               (get_op op <> Rd ==> (get_rval (app_op st op) = spec op tr)))
+#set-options "--z3rlimit 1000000"
+let prop_spec tr st op = ()
+
+instance orset : mrdt s op rval = {
   Library.init = init;
+  Library.spec = spec;
   Library.sim = sim;
   Library.pre_cond_op = pre_cond_op;
   Library.app_op = app_op;
@@ -230,5 +309,6 @@ instance _ : mrdt s op = {
   Library.merge1 = merge1;
   Library.merge = merge;
   Library.prop_merge = prop_merge;
+  Library.prop_spec = prop_spec;
   Library.convergence = convergence
 }
