orset_bst.fst
@@ -18,21 +18,21 @@ let rec memt1 x t =
   | Leaf -> false
   | Node n t1 t2 -> x = n || memt1 x t1 || memt1 x t2
 
-val member_id : id:nat 
+val member_id_s : id:nat 
               -> t:tree
               -> Tot (b:bool {(exists ele. memt1 (id,ele) t) <==> b = true})
-let rec member_id id t =
+let rec member_id_s id t =
   match t with
   | Leaf -> false
-  | Node (id1,_) t1 t2 -> id = id1 || member_id id t1 || member_id id t2
+  | Node (id1,_) t1 t2 -> id = id1 || member_id_s id t1 || member_id_s id t2
 
-val member_ele : ele:nat 
+val member_ele_s : ele:nat 
                -> t:tree 
                -> Tot (b:bool {(exists id. memt1 (id,ele) t) <==> b = true})
-let rec member_ele ele t =
+let rec member_ele_s ele t =
   match t with
   | Leaf -> false
-  | Node (_,ele1) t1 t2 -> ele = ele1 || member_ele ele t1 || member_ele ele t2
+  | Node (_,ele1) t1 t2 -> ele = ele1 || member_ele_s ele t1 || member_ele_s ele t2
 
 val forallt : p:((nat * nat) -> Tot bool)
             -> t:tree 
@@ -42,23 +42,23 @@ let rec forallt p t =
   | Leaf -> true
   | Node n t1 t2 -> p n && forallt p t1 && forallt p t2
 
-val unique_id : t:tree -> Tot bool
-let rec unique_id t =
+val unique_id_s : t:tree -> Tot bool
+let rec unique_id_s t =
   match t with
   |Leaf -> true
-  |Node (id,ele) t1 t2 -> not (member_id id t1) && not (member_id id t2) &&
-                         forallt (fun e -> not (member_id (fst e) t2)) t1 && 
-                         forallt (fun e -> not (member_id (fst e) t1)) t2 &&
-                         unique_id t1 && unique_id t2 
+  |Node (id,ele) t1 t2 -> not (member_id_s id t1) && not (member_id_s id t2) &&
+                         forallt (fun e -> not (member_id_s (fst e) t2)) t1 && 
+                         forallt (fun e -> not (member_id_s (fst e) t1)) t2 &&
+                         unique_id_s t1 && unique_id_s t2 
 
-val unique_ele : t:tree -> Tot bool
-let rec unique_ele t =
+val unique_ele_s : t:tree -> Tot bool
+let rec unique_ele_s t =
   match t with
   |Leaf -> true
-  |Node (id,ele) t1 t2 -> not (member_ele ele t1) && not (member_ele ele t2) &&
-                           forallt (fun e -> not (member_ele (snd e) t2)) t1 && 
-                           forallt (fun e -> not (member_ele (snd e) t1)) t2 &&
-                           unique_ele t1 && unique_ele t2
+  |Node (id,ele) t1 t2 -> not (member_ele_s ele t1) && not (member_ele_s ele t2) &&
+                           forallt (fun e -> not (member_ele_s (snd e) t2)) t1 && 
+                           forallt (fun e -> not (member_ele_s (snd e) t1)) t2 &&
+                           unique_ele_s t1 && unique_ele_s t2
 
 val is_bst : tree -> Tot bool
 let rec is_bst t =
@@ -73,14 +73,16 @@ let rec size t1 =
   |Leaf -> 0
   |Node _ t1 t2 -> 1 + size t1 + size t2
 
-type s = tree1:tree {is_bst tree1 /\ unique_id tree1}
+type s = tree1:tree {is_bst tree1 /\ unique_id_s tree1}
+
+type rval = O.rval
 
 val init : s
 let init = Leaf
 
 type op = O.op
 
-val help : t1:s -> Lemma (ensures unique_ele t1)
+val help : t1:s -> Lemma (ensures unique_ele_s t1)
                   [SMTPat (is_bst t1)]
 #set-options "--z3rlimit 1000000"
 let rec help tr = 
@@ -103,7 +105,7 @@ let ge n1 n2 = (snd n1 > snd n2 && fst n1 <> fst n2) || n1 = n2
 
 val find_max : t1:tree {Node? t1}
              -> Pure (nat * nat)
-               (requires (is_bst t1 /\ unique_id t1))
+               (requires (is_bst t1 /\ unique_id_s t1))
                (ensures (fun r -> (forallt (ge r) t1) /\ memt1 r t1))
 let rec find_max t1 =
   match t1 with
@@ -116,8 +118,8 @@ val delete_ele : x:nat
                -> t1:s
                -> Pure s
                  (requires true)
-                 (ensures (fun r -> (forall e. memt1 e r <==> (memt e t1) /\ snd e <> x) /\ not (member_ele x r) /\ 
-                                   is_bst r /\ unique_id r)) 
+                 (ensures (fun r -> (forall e. memt1 e r <==> (memt e t1) /\ snd e <> x) /\ not (member_ele_s x r) /\ 
+                                   is_bst r /\ unique_id_s r)) 
                  (decreases (size t1))
 
 #set-options "--z3rlimit 1000000"
@@ -158,13 +160,13 @@ val update : ele:nat
            -> id:nat
            -> t1:s
            -> Pure tree
-             (requires not (member_id id t1))
+             (requires not (member_id_s id t1))
              (ensures (fun res -> (forall e. memt e t1 /\ snd e <> ele <==> memt1 e res /\ snd e <> ele) /\
-                               (forall e. memt1 e res /\ fst e <> id /\ member_id (fst e) res <==> 
-                                     memt e t1 /\ snd e <> ele /\ member_id (fst e) t1) /\
-                               (forall e. member_ele e t1 \/ e = ele <==> member_ele e res) /\
+                               (forall e. memt1 e res /\ fst e <> id /\ member_id_s (fst e) res <==> 
+                                     memt e t1 /\ snd e <> ele /\ member_id_s (fst e) t1) /\
+                               (forall e. member_ele_s e t1 \/ e = ele <==> member_ele_s e res) /\
                                (forall e. memt1 e res /\ e <> (id,ele) <==> memt e t1 /\ snd e <> ele) /\ 
-                                     memt1 (id,ele) res /\ is_bst res /\ unique_id res))
+                                     memt1 (id,ele) res /\ is_bst res /\ unique_id_s res))
 
 #set-options "--z3rlimit 1000000"
 let rec update ele id tr =
@@ -174,30 +176,69 @@ let rec update ele id tr =
                               else if ele < ele1 then (Node (id1,ele1) (update ele id t1) t2)
                                  else Node (id1,ele1) t1 (update ele id t2)
 
-let pre_cond_op s1 op = not (member_id (get_id op) s1)
+let pre_cond_op s1 op = not (member_id_s (get_id op) s1)
+
+val appendt : l1:O.s
+            -> l2:O.s
+            -> Pure O.s
+              (requires (forall e. O.member_ele_s e l1 ==> not (O.member_ele_s e l2)) /\
+                        (forall e. O.member_id_s e l1 ==> not (O.member_id_s e l2)))
+              (ensures (fun res -> (forall e. mem e res <==> mem e l1 \/ mem e l2) /\
+                                (forall e. O.member_id_s e res <==> O.member_id_s e l1 \/ O.member_id_s e l2) /\
+                                (forall e. O.member_ele_s e res <==> O.member_ele_s e l1 \/ O.member_ele_s e l2)))
+let rec appendt l1 l2 =
+  match l1,l2 with
+  |[],[] -> []
+  |x::xs,_ -> x::(appendt xs l2)
+  |[],_ -> l2
+
+val flatten : tree1:s
+            -> Pure O.s
+              (requires true)
+              (ensures (fun res -> (forall e. memt e tree1 <==> mem e res) /\
+                                (forall e. member_ele_s e tree1 <==> O.member_ele_s e res) /\
+                                (forall e. member_id_s e tree1 <==> O.member_id_s e res)))
+              (decreases (size tree1))
+
+#set-options "--z3rlimit 1000000"
+let rec flatten t =
+  match t with
+  |Leaf -> []
+  |Node n t1 t2 -> assert ((forall e. O.member_ele_s e (flatten t1) ==> not (O.member_ele_s e (flatten t2))) /\
+                          (forall e. O.member_id_s e (flatten t1) ==> not (O.member_id_s e (flatten t2))) /\
+                           not (O.member_id_s (fst n) (flatten t1)) /\
+                           not (O.member_ele_s (snd n) (flatten t1)) /\
+                           not (O.member_id_s (fst n) (flatten t2)) /\
+                           not (O.member_ele_s (snd n) (flatten t2)));
+                  assert (not (O.member_id_s (fst n) (appendt (flatten t1) (flatten t2))) /\
+                          not (O.member_ele_s (snd n) (appendt (flatten t1) (flatten t2))));
+                  n::(appendt (flatten t1) (flatten t2))
 
 val app_op : s1:s
            -> op1:(nat * op)
-           -> Pure s
+           -> Pure (s * rval)
              (requires pre_cond_op s1 op1)
-             (ensures (fun res -> (O.opa op1 ==> (forall e. memt e s1 /\ snd e <> O.get_ele op1 <==> 
-                                                   memt e res /\ snd e <> O.get_ele op1) /\
-                               (forall e. memt e res /\ fst e <> get_id op1 /\ member_id (fst e) res <==> 
-                                     memt e s1 /\ snd e <> O.get_ele op1 /\ member_id (fst e) s1) /\
-                               (forall e. member_ele e s1 \/ e = O.get_ele op1 <==> member_ele e res) /\
-                               (forall e. memt e res /\ e <> ((get_id op1), (O.get_ele op1)) <==> 
+             (ensures (fun res -> (O.opa op1 ==> (get_rval res = O.Bot) /\ (forall e. memt e s1 /\ snd e <> O.get_ele op1 <==> 
+                                                   memt e (get_st res) /\ snd e <> O.get_ele op1) /\
+                               (forall e. memt e (get_st res) /\ fst e <> get_id op1 /\ member_id_s (fst e) (get_st res) <==> 
+                                     memt e s1 /\ snd e <> O.get_ele op1 /\ member_id_s (fst e) s1) /\
+                               (forall e. member_ele_s e s1 \/ e = O.get_ele op1 <==> member_ele_s e (get_st res)) /\
+                               (forall e. memt e (get_st res) /\ e <> ((get_id op1), (O.get_ele op1)) <==> 
                                      memt e s1 /\ snd e <> O.get_ele op1) /\
-                                     memt ((get_id op1), (O.get_ele op1)) res) /\
-                               (O.opr op1 ==> (forall e. memt e res <==> memt e s1 /\ snd e <> O.get_ele op1))))
+                                     memt ((get_id op1), (O.get_ele op1)) (get_st res)) /\
+                                  (O.opr op1 ==> (get_rval res = O.Bot) /\ (forall e. memt e (get_st res) <==> memt e s1 /\ snd e <> O.get_ele op1)) /\ (get_op op1 = O.Rd ==> get_rval res = O.Val (O.get_set_s (flatten s1)) /\ get_st res = s1)))
 
 let app_op s1 op =
-  if O.opa op then update (O.get_ele op) (get_id op) s1 else delete_ele (O.get_ele op) s1
+  match op with
+  |(_, O.Add _) -> (update (O.get_ele op) (get_id op) s1, O.Bot)
+  |(_, O.Rem _) -> (delete_ele (O.get_ele op) s1, O.Bot)
+  |(_, O.Rd) -> (s1, O.Val (O.get_set_s (flatten s1)))
 
 val insert : x:(nat * nat)
            -> t1:s
            -> Pure tree
-             (requires (not (memt x t1) /\ not (member_id (fst x) t1) /\ not (member_ele (snd x) t1)))
-             (ensures (fun r -> is_bst r /\ (forall y. memt1 y r <==> (memt y t1 \/ x = y)) /\ unique_id r))
+             (requires (not (memt x t1) /\ not (member_id_s (fst x) t1) /\ not (member_ele_s (snd x) t1)))
+             (ensures (fun r -> is_bst r /\ (forall y. memt1 y r <==> (memt y t1 \/ x = y)) /\ unique_id_s r))
              (decreases (size t1))
 
 #set-options "--z3rlimit 1000000"
@@ -211,8 +252,8 @@ let rec insert x t =
 val totree1 : s1:O.s
             -> acc:s
             -> Pure s
-              (requires (forall e. member_id e acc ==> not (O.member_id e s1)) /\
-                        (forall e. member_ele e acc ==> not (O.member_ele e s1)))
+              (requires (forall e. member_id_s e acc ==> not (O.member_id_s e s1)) /\
+                        (forall e. member_ele_s e acc ==> not (O.member_ele_s e s1)))
               (ensures (fun t1 -> (forall e. memt e t1 <==> mem e s1 \/ memt e acc)))
 
 #set-options "--z3rlimit 1000000"
@@ -222,50 +263,14 @@ let rec totree1 l acc =
   |x::xs -> totree1 xs (insert x acc)
 
 val totree : l:O.s -> t1:s {(forall e. memt e t1 <==> mem e l) /\
-                           (forall e. member_ele e t1 <==> O.member_ele e l) /\
-                           (forall e. member_id e t1 <==> O.member_id e l)}
+                           (forall e. member_ele_s e t1 <==> O.member_ele_s e l) /\
+                           (forall e. member_id_s e t1 <==> O.member_id_s e l)}
 let totree l = totree1 l Leaf
 
 val lt : n1:(nat * nat) 
        -> n2:(nat * nat)
        -> Tot (b:bool)
 let lt (id,ele) (id1,ele1) = (ele < ele1 && id <> id1)
-
-val appendt : l1:O.s
-            -> l2:O.s
-            -> Pure O.s
-              (requires (forall e. O.member_ele e l1 ==> not (O.member_ele ( e) l2)) /\
-                        (forall e. O.member_id e l1 ==> not (O.member_id ( e) l2)))
-              (ensures (fun res -> (forall e. mem e res <==> mem e l1 \/ mem e l2) /\
-                                (forall e. O.member_id e res <==> O.member_id e l1 \/ O.member_id e l2) /\
-                                (forall e. O.member_ele e res <==> O.member_ele e l1 \/ O.member_ele e l2)))
-let rec appendt l1 l2 =
-  match l1,l2 with
-  |[],[] -> []
-  |x::xs,_ -> x::(appendt xs l2)
-  |[],_ -> l2
-
-val flatten : tree1:s
-            -> Pure O.s
-              (requires true)
-              (ensures (fun res -> (forall e. memt e tree1 <==> mem e res) /\
-                                (forall e. member_ele e tree1 <==> O.member_ele e res) /\
-                                (forall e. member_id e tree1 <==> O.member_id e res)))
-              (decreases (size tree1))
-
-#set-options "--z3rlimit 1000000"
-let rec flatten t =
-  match t with
-  |Leaf -> []
-  |Node n t1 t2 -> assert ((forall e. O.member_ele e (flatten t1) ==> not (O.member_ele ( e) (flatten t2))) /\
-                          (forall e. O.member_id e (flatten t1) ==> not (O.member_id ( e) (flatten t2))) /\
-                           not (O.member_id (fst n) ( (flatten t1) )) /\
-                           not (O.member_ele (snd n) ( (flatten t1) )) /\
-                           not (O.member_id (fst n) ( (flatten t2) )) /\
-                           not (O.member_ele (snd n) ( (flatten t2) )));
-                  assert (not (O.member_id (fst n) (appendt (flatten t1) (flatten t2))) /\
-                          not (O.member_ele (snd n) (appendt (flatten t1) (flatten t2))));
-                  n::(appendt (flatten t1) (flatten t2))
 
 val fst : (nat * nat) -> nat
 let fst (id,ele) = id
@@ -280,31 +285,31 @@ val sim : tr:ae op
                                      not (tr.vis a r)) ==> fst e >= get_id a) /\ 
                  (mem ((fst e), O.Add (snd e)) tr.l /\
   (forall r. mem r tr.l /\ O.opr r /\ O.get_ele r = snd e /\ fst e <> get_id r ==> not (tr.vis ((fst e), O.Add (snd e)) r)))) /\
-                 (forall a. mem a tr.l /\ O.opa a ==> (forall r. mem r tr.l /\ O.opr r /\ O.get_ele a = O.get_ele r /\ get_id a <> get_id r ==> not (tr.vis a r)) ==> member_ele (O.get_ele a) s1))})
+                 (forall a. mem a tr.l /\ O.opa a ==> (forall r. mem r tr.l /\ O.opr r /\ O.get_ele a = O.get_ele r /\ get_id a <> get_id r ==> not (tr.vis a r)) ==> member_ele_s (O.get_ele a) s1))})
 
 #set-options "--z3rlimit 1000000"
-let sim tr s1 = 
-  let lsta = (filter (fun a -> O.opa a) tr.l) in
-  let lstr = (filter (fun r -> O.opr r) tr.l) in
-  let lst = filter (fun a -> not (existsb (fun r -> get_id a <> get_id r && 
+let sim tr s1 = O.sim tr (flatten s1)
+  (*)let lsta = (O.filtero (fun a -> O.opa a) tr.l) in
+  let lstr = (O.filtero (fun r -> O.opr r) tr.l) in
+  let lst = O.filtero (fun a -> not (existsb (fun r -> get_id a <> get_id r && 
             O.get_ele r = O.get_ele a && tr.vis a r) lstr)) lsta in
 
-  (forallt (fun e -> (forallb (fun a -> fst e >= get_id a) (filter (fun a -> O.get_ele a = snd e) lst)) &&
+  (forallt (fun e -> (O.forallo (fun a -> fst e >= get_id a) (O.filtero (fun a -> O.get_ele a = snd e) lst)) &&
                   (mem ((fst e), O.Add (snd e)) tr.l &&
                    not (existsb (fun r -> fst e <> get_id r && tr.vis ((fst e), O.Add (snd e)) r ) 
                   (filter (fun r -> snd e = O.get_ele r) lstr)))) s1) &&
-  (forallb (fun a -> member_ele (O.get_ele a) s1) lst)
+  (forallb (fun a -> member_ele_s (O.get_ele a) s1) lst)*)
 
 val diff : a:s
          -> l:s
          -> Pure s
            (requires true)
            (ensures (fun d -> (forall e. memt e d <==> memt e a /\ not (memt e l)) /\
-                           (forall e. memt e d /\ member_id (fst e) d <==> 
-                                 memt e a /\ member_id (fst e) a /\ not (memt e l)) /\
-                           (forall e. memt e d  /\ member_ele (snd e) d <==> 
-                                 memt e a /\ member_ele (snd e) a /\ not (memt e l)) /\
-                           (forall e. memt e a /\ memt e l ==> not (member_ele (snd e) d) /\ not (member_id (fst e) d))))
+                           (forall e. memt e d /\ member_id_s (fst e) d <==> 
+                                 memt e a /\ member_id_s (fst e) a /\ not (memt e l)) /\
+                           (forall e. memt e d  /\ member_ele_s (snd e) d <==> 
+                                 memt e a /\ member_ele_s (snd e) a /\ not (memt e l)) /\
+                           (forall e. memt e a /\ memt e l ==> not (member_ele_s (snd e) d) /\ not (member_id_s (fst e) d))))
            (decreases %[l;a])
 let diff a l =
   totree (O.diff (flatten a) (flatten l))
@@ -356,11 +361,11 @@ val prop_oper : tr:ae op
               -> op:(nat * op)
               -> Lemma (requires (sim tr st) /\ (not (mem_id (get_id op) tr.l)) /\
                                 (forall e. mem e tr.l ==> get_id e < get_id op) /\ get_id op > 0)
-                      (ensures (sim (append tr op) (app_op st op)))
+                      (ensures (sim (append tr op) (get_st (app_op st op))))
 
 #set-options "--z3rlimit 10000000"
 let prop_oper tr st op =
-  assert (not (member_id (get_id op) st));
+  assert (not (member_id_s (get_id op) st));
   O.prop_oper tr (flatten st) op
 
 val convergence : tr:ae op
@@ -371,8 +376,20 @@ val convergence : tr:ae op
 let convergence tr a b =
   O.convergence tr (flatten a) (flatten b)
 
-instance _ : mrdt s op = {
+val prop_spec : tr:ae op
+              -> st:s
+              -> op:(nat * op)
+              -> Lemma (requires (sim tr st) /\ (not (mem_id (get_id op) tr.l)) /\
+                                (forall e. mem e tr.l ==> get_id e < get_id op) /\ get_id op > 0)
+                      (ensures (get_op op = O.Rd ==> (forall e. mem e (O.extract (get_rval (app_op st op))) <==>
+                                               mem e (O.extract (O.spec op tr)))) /\
+                               (get_op op <> O.Rd ==> (get_rval (app_op st op) = O.spec op tr)))
+#set-options "--z3rlimit 1000000"
+let prop_spec tr st op = ()
+
+instance orset_bst : mrdt s op rval = {
   Library.init = init;
+  Library.spec = O.spec;
   Library.sim = sim;
   Library.pre_cond_op = pre_cond_op;
   Library.app_op = app_op;
@@ -382,8 +399,10 @@ instance _ : mrdt s op = {
   Library.merge1 = merge1;
   Library.merge = merge;
   Library.prop_merge = prop_merge;
+  Library.prop_spec = prop_spec;
   Library.convergence = convergence
 }
+
 
 
 (******************* Height-balanced BST ************************)
