orset_space.fst
@@ -3,81 +3,110 @@ open FStar.List.Tot
 
 open Library
 
-val member_id : id:nat 
-              -> l:list (nat * nat)
-              -> Tot (b:bool{(exists n. mem (id,n) l) <==> b=true})
-let rec member_id n l =
-  match l with
-  |[] -> false
-  |(id,_)::xs -> (n = id) || member_id n xs
+  val member_id_s : id:nat 
+                  -> l:list (nat * nat)
+                  -> Tot (b:bool{(exists n. mem (id,n) l) <==> b=true})
+  let rec member_id_s n l =
+    match l with
+    |[] -> false
+    |(id,_)::xs -> (n = id) || member_id_s n xs
 
-val unique_id : l:list (nat * nat)
-              -> Tot bool
-let rec unique_id l =
-  match l with
-  |[] -> true
-  |(id,_)::xs -> not (member_id id xs) && unique_id xs
+  val unique_id_s : l:list (nat * nat)
+                  -> Tot bool
+  let rec unique_id_s l =
+    match l with
+    |[] -> true
+    |(id,_)::xs -> not (member_id_s id xs) && unique_id_s xs
 
-val member_ele : ele:nat
-               -> l:list (nat * nat)
-               -> Tot (b:bool{(exists id. mem (id,ele) l) <==> b=true})
-let rec member_ele ele l =
-  match l with
-  |[] -> false
-  |(_,ele1)::xs -> (ele = ele1) || member_ele ele xs
+  val member_ele_s : ele:nat
+                   -> l:list (nat * nat)
+                   -> Tot (b:bool{(exists id. mem (id,ele) l) <==> b=true})
+  let rec member_ele_s ele l =
+    match l with
+    |[] -> false
+    |(_,ele1)::xs -> (ele = ele1) || member_ele_s ele xs
 
-val unique_ele : l:list (nat * nat)
-               -> Tot bool
-let rec unique_ele l =
-  match l with
-  |[] -> true
-  |(_,ele)::xs -> not (member_ele ele xs) && unique_ele xs
+  val unique_ele_s : l:list (nat * nat)
+                   -> Tot bool
+  let rec unique_ele_s l =
+    match l with
+    |[] -> true
+    |(_,ele)::xs -> not (member_ele_s ele xs) && unique_ele_s xs
 
-type s = l:list (nat (*unique id*) * nat (*unique element*)) {unique_id l /\ unique_ele l}
+  type s = l:list (nat (*unique id*) * nat (*unique element*)) {unique_id_s l /\ unique_ele_s l}
+
+type rval = |Val : list nat -> rval
+            |Bot
 
 val init : s
 let init = []
 
-val filter_uni : f:((nat * nat) -> bool)
-               -> l:list (nat * nat) 
-               -> Lemma (requires (unique_id l /\ unique_ele l))
-                       (ensures (unique_id (filter f l) /\ unique_ele (filter f l)))
-                               [SMTPat (filter f l)]
+val mem_ele_s : ele:nat -> s1:s -> Tot (b:bool {b = true <==> (exists id. mem (id,ele) s1)})
+let rec mem_ele_s ele s =
+  match s with
+  |[] -> false
+  |(_,ele1)::xs -> ele = ele1 || mem_ele_s ele xs
 
-#set-options "--z3rlimit 1000000"
-let rec filter_uni f l =
-  match l with
-  |[] -> ()
-  |x::xs -> filter_uni f xs
+  val filter_uni : f:((nat * nat) -> bool)
+                 -> l:list (nat * nat) 
+                 -> Lemma (requires (unique_id_s l /\ unique_ele_s l))
+                         (ensures (unique_id_s (filter f l) /\ unique_ele_s (filter f l)))
+                                  [SMTPat (filter f l)]
+
+  #set-options "--z3rlimit 1000000"
+  let rec filter_uni f l =
+    match l with
+    |[] -> ()
+    |x::xs -> filter_uni f xs
 
 type op =
   |Add : nat (*element*) -> op
   |Rem : nat (*element*) -> op
+  |Rd
 
-val get_ele : op1:(nat * op) -> Tot (ele:nat {(exists id. op1 = (id, Add ele) \/ op1 = (id, Rem ele))})
-let get_ele op =
-  match op with
-  |(_, (Add ele)) -> ele
-  |(_, (Rem ele)) -> ele
-
-val opa : op1:(nat * op) -> Tot (b:bool {b = true <==> (exists id ele. op1 = (id, Add ele))})
+val opa : op1:(nat * op) -> Tot (b:bool {b = true <==> (exists id ele. op1 = (id, Add ele)) /\ get_op op1 <> Rd})
 let opa op1 =
   match op1 with
   |(_, Add _) -> true
   |_ -> false
 
-val opr : op1:(nat * op) -> Tot (b:bool {b = true <==> (exists id ele. op1 = (id, Rem ele))})
-let opr op1 = not (opa op1)
+val opr : op1:(nat * op) -> Tot (b:bool {b = true <==> (exists id ele. op1 = (id, Rem ele)) /\ get_op op1 <> Rd})
+let opr op1 =
+  match op1 with
+  |(_, Rem _) -> true
+  |_ -> false
+
+val mem_ele : ele:nat -> l:list (nat * op) -> Tot (b:bool {b = true <==> (exists id. mem (id, (Add ele)) l) \/ (exists id. mem (id, (Rem ele)) l)})
+let rec mem_ele ele l =
+  match l with
+  |[] -> false
+  |(_, (Add ele1))::xs -> ele = ele1 || mem_ele ele xs
+  |(_, (Rem ele1))::xs -> ele = ele1 || mem_ele ele xs
+  |(_, Rd)::xs -> mem_ele ele xs
+
+val get_ele : op1:(nat * op){get_op op1 <> Rd} -> Tot (ele:nat {(exists id. op1 = (id, Add ele) \/ op1 = (id, Rem ele))})
+let get_ele op =
+  match op with
+  |(_, (Add ele)) -> ele
+  |(_, (Rem ele)) -> ele
+
+let pre_cond_op s1 op = not (member_id_s (get_id op) s1)
+
+val get_set_s : s1:s -> Tot (l:list nat {(forall e. mem e l <==> mem_ele_s e s1)})
+let rec get_set_s s1 = 
+  match s1 with
+  |[] -> []
+  |(_,ele)::xs -> if mem_ele_s ele xs then get_set_s xs else ele::get_set_s xs
 
 val update : s1:s
            -> ele:nat
            -> id:nat
            -> Pure s
-               (requires (member_ele ele s1) /\ not (member_id id s1))
+               (requires (member_ele_s ele s1) /\ not (member_id_s id s1))
                (ensures (fun u -> (forall e. mem e s1 /\ snd e <> ele <==> mem e u /\ snd e <> ele) /\
-                               (forall e. mem e u /\ fst e <> id /\ member_id (fst e) u <==> 
-                                     mem e s1 /\ snd e <> ele /\ member_id (fst e) s1) /\
-                                (forall e. member_ele e s1 <==> member_ele e u) /\
+                               (forall e. mem e u /\ fst e <> id /\ member_id_s (fst e) u <==> 
+                                     mem e s1 /\ snd e <> ele /\ member_id_s (fst e) s1) /\
+                                (forall e. member_ele_s e s1 <==> member_ele_s e u) /\
                                 (forall e. mem e u /\ e <> (id,ele) <==> mem e s1 /\ snd e <> ele) /\ mem (id,ele) u))
                                 (decreases s1)
 let rec update s1 ele id =
@@ -88,45 +117,100 @@ let rec update s1 ele id =
 val remove_ele : s1:s
                  -> ele:nat
                  -> Pure s
-                 (requires (member_ele ele s1))
+                 (requires (member_ele_s ele s1))
                  (ensures (fun u -> (forall e. mem e s1 /\ snd e <> ele <==> mem e u)))
                  (decreases s1)
 let rec remove_ele s1 ele =
   match s1 with
   |[] -> []
   |(id1,ele1)::xs -> if ele = ele1 then xs else (id1,ele1):: remove_ele xs ele
-
-let pre_cond_op s1 op = not (member_id (get_id op) s1)
-
+  
 val app_op : s1:s
            -> op:(nat * op)
-           -> Pure s
+           -> Pure (s * rval)
              (requires pre_cond_op s1 op)
-             (ensures (fun res -> (opa op ==> (forall e. mem e s1 /\ snd e <> get_ele op <==> mem e res /\ snd e <> get_ele op) /\
-                                          (forall e. mem e res /\ fst e <> get_id op /\ member_id (fst e) res <==> mem e s1 /\ snd e <> get_ele op /\ member_id (fst e) s1) /\
-                                          (forall e. member_ele e s1 \/ e = get_ele op <==> member_ele e res) /\
-                                          (forall e. mem e res /\ e <> ((get_id op), (get_ele op)) <==> mem e s1 /\ snd e <> get_ele op) /\
-                                            mem ((get_id op), (get_ele op)) res) /\
-                               (opr op ==> (forall e. mem e res <==> mem e s1 /\ snd e <> get_ele op))))
+             (ensures (fun res -> (opa op ==> (get_rval res = Bot) /\ (forall e. mem e s1 /\ snd e <> get_ele op <==> mem e (get_st res) /\ snd e <> get_ele op) /\
+                                          (forall e. mem e (get_st res) /\ fst e <> get_id op /\ member_id_s (fst e) (get_st res) <==> mem e s1 /\ snd e <> get_ele op /\ member_id_s (fst e) s1) /\
+                                          (forall e. member_ele_s e s1 \/ e = get_ele op <==> member_ele_s e (get_st res)) /\
+                                          (forall e. mem e (get_st res) /\ e <> ((get_id op), (get_ele op)) <==> mem e s1 /\ snd e <> get_ele op) /\
+                                            mem ((get_id op), (get_ele op)) (get_st res)) /\
+                               (opr op ==> (get_rval res = Bot) /\ (forall e. mem e (get_st res) <==> mem e s1 /\ snd e <> get_ele op)) /\ (get_op op = Rd ==> get_rval res = Val (get_set_s s1) /\ get_st res = s1)))
 let app_op s1 op =
-  if (opa op) 
-    then (if member_ele (get_ele op) s1 then (update s1 (get_ele op) (get_id op))
-      else ((get_id op),(get_ele op))::s1) 
-        else (if member_ele (get_ele op) s1 then (remove_ele s1 (get_ele op)) else s1)
+  match op with
+  |(_, Add _) -> if member_ele_s (get_ele op) s1 then (update s1 (get_ele op) (get_id op), Bot)
+                    else (((get_id op),(get_ele op))::s1, Bot)
+  |(_, Rem _) -> if member_ele_s (get_ele op) s1 then (remove_ele s1 (get_ele op), Bot) else (s1, Bot)
+  |(_, Rd) -> (s1, Val (get_set_s s1))
 
 val filter_uni1 : f:((nat * op) -> bool)
                 -> l:list (nat * op) 
-                -> Lemma (requires (Library.unique_id l))
-                        (ensures (Library.unique_id (filter f l)))
-                           [SMTPat (filter f l)]
+                -> Lemma (requires (unique_id l))
+                        (ensures (unique_id (filter f l)))
+                        [SMTPat (filter f l)]
 let rec filter_uni1 f l = 
   match l with
   |[] -> ()
   |x::xs -> filter_uni1 f xs
 
-val fst : nat * nat -> nat
+val except : f:((nat * op) -> bool)
+           -> l:list (nat * op) {unique_id l}
+           -> Tot (l1:list (nat * op) {(forall e. mem e l1 <==> mem e l /\ not (f e)) /\ unique_id l1})
+let rec except f l =
+  match l with
+  |[] -> []
+  |hd::tl -> if not (f hd) then hd::(except f tl) else except f tl
+
+val filtero : f:((nat * op) -> bool)
+             -> l:list (nat * op) {unique_id l}
+             -> Tot (l1:list (nat * op) {(forall e. mem e l1 <==> mem e l /\ (f e)) /\ unique_id l1})
+let rec filtero f l =
+    match l with
+    |[] -> []
+    |hd::tl -> if (f hd) then hd::(filtero f tl) else filtero f tl
+
+val existsb : f:((nat * op) -> bool)
+            -> l:list (nat * op)
+            -> Tot (b:bool{(exists e. mem e l /\ f e) <==> b = true})
+let rec existsb f l =
+    match l with
+    |[] -> false
+    |hd::tl -> if f hd then true else existsb f tl
+
+val get_set : tr:list (nat * op){unique_id tr} -> Tot (s1:list nat {(forall e. mem e s1 <==> mem_ele e tr)})
+let rec get_set l =
+  match l with
+  |[] -> []
+  |(_, Add x)::xs -> if mem_ele x xs then get_set xs else x::(get_set xs)
+  |(_, Rem x)::xs -> if mem_ele x xs then get_set xs else x::(get_set xs)
+  |(_, Rd)::xs -> get_set xs
+
+val extract : r:rval {exists v. r = Val v} -> list nat
+let extract (Val s) = s
+
+val forallo : f:((nat * op) -> bool)
+            -> l:list (nat * op)
+            -> Tot (b:bool{(forall e. mem e l ==> f e) <==> b = true})
+let rec forallo f l =
+  match l with
+  |[] -> true
+  |hd::tl -> if f hd then forallo f tl else false
+
+val spec : o:(nat * op) -> tr:ae op
+         -> Tot (r:rval {(get_op o = Rd ==> r <> Bot /\ (forall e. mem e (extract r) <==> (exists id. mem (id, Add e) tr.l /\
+                                    (forall r. mem r tr.l /\ id <> get_id r /\ opr r ==>
+                                              not (e = get_ele r && (tr.vis (id, Add e) r)))))) /\
+                       (opa o ==> r = Bot) /\ (opr o ==> r = Bot)})
+let spec o tr =
+  match o with
+  |(_, Add _) -> Bot
+  |(_, Rem _) -> Bot
+  |(_, Rd) -> let lsta = (filter (fun a -> opa a) tr.l) in
+  let lstr = (filter (fun r -> opr r) tr.l) in
+  let lst = except (fun a -> get_op a <> Rd && opa a && (existsb (fun r -> get_op r <> Rd && get_op a <> Rd && opa a && opr r && get_id a <> get_id r && get_ele r = get_ele a && tr.vis a r) lstr)) lsta in Val (get_set lst)
+
+val fst : (nat * nat) -> nat
 let fst (id,ele) = id
-val snd : nat * nat -> nat
+val snd : (nat * nat) -> nat
 let snd (id,ele) = ele
 
 #set-options "--query_stats"
@@ -136,27 +220,27 @@ val sim : tr:ae op
                        (forall r. mem r tr.l /\ opr r /\ get_ele a = get_ele r /\ get_id a <> get_id r ==> 
                         not (tr.vis a r)) ==> fst e >= get_id a) /\ 
                        (mem ((fst e), Add (snd e)) tr.l /\
-              (forall r. mem r tr.l /\ opr r /\ get_ele r = snd e ==> not (fst e <> get_id r && tr.vis ((fst e), Add (snd e)) r)))) /\
-                 (forall a. mem a tr.l /\ opa a ==> (forall r. mem r tr.l /\ opr r /\ get_ele a = get_ele r /\ get_id a <> get_id r ==> not (tr.vis a r)) ==> member_ele (get_ele a) s1))})
+   (forall r. mem r tr.l /\ opr r /\ get_ele r = snd e /\ fst e <> get_id r ==> not (tr.vis ((fst e), Add (snd e)) r)))) /\
+                 (forall a. mem a tr.l /\ opa a ==> (forall r. mem r tr.l /\ opr r /\ get_ele a = get_ele r /\ get_id a <> get_id r ==> not (tr.vis a r)) ==> member_ele_s (get_ele a) s1))})
 
 #set-options "--z3rlimit 1000000"
 let sim tr s1 = 
-  let lsta = (filter (fun a -> opa a) tr.l) in
-  let lstr = (filter (fun r -> opr r) tr.l) in
-  let lst = filter (fun a -> not (existsb (fun r -> get_id a <> get_id r && get_ele r = get_ele a && tr.vis a r) lstr)) lsta in
+  let lsta = (filtero (fun a -> opa a) tr.l) in
+  let lstr = (filtero (fun r -> opr r) tr.l) in
+  let lst = filtero (fun a -> get_op a <> Rd && opa a && not (existsb (fun r -> get_op r <> Rd && get_op a <> Rd && opa a && opr r && get_id a <> get_id r && get_ele r = get_ele a && tr.vis a r) lstr)) lsta in
 
-  (forallb (fun e -> (forallb (fun a -> fst e >= get_id a) (filter (fun a -> get_ele a = snd e) lst)) &&
+  (forallb (fun e -> (forallo (fun a -> fst e >= get_id a) (filtero (fun a -> get_op a <> Rd && get_ele a = snd e) lst)) &&
                   (mem ((fst e), Add (snd e)) tr.l && 
-                  not (existsb (fun r -> tr.vis ((fst e), Add (snd e)) r ) 
-                  (filter (fun r -> snd e = get_ele r && fst e <> get_id r) lstr)))) s1) &&
-  (forallb (fun a -> member_ele (get_ele a) s1) lst)
+                  not (existsb (fun r -> tr.vis ((fst e), Add (snd e)) r) 
+                  (filtero (fun r -> get_op r <> Rd && snd e = get_ele r && fst e <> get_id r) lstr)))) s1) &&
+  (forallo (fun a -> get_op a <> Rd && member_ele_s (get_ele a) s1) lst)
 
 val prop_oper : tr:ae op
               -> st:s
               -> op:(nat * op)
               -> Lemma (requires (sim tr st) /\ (not (mem_id (get_id op) tr.l)) /\
                                 (forall e. mem e tr.l ==> get_id e < get_id op) /\ get_id op > 0)
-                      (ensures (sim (append tr op) (app_op st op)))
+                      (ensures (sim (append tr op) (get_st (app_op st op))))
 
 #set-options "--z3rlimit 1000000"
 let prop_oper tr st op = ()
@@ -173,9 +257,9 @@ val remove : l:s
            -> Pure s 
                (requires (mem ele l))
                (ensures (fun res -> (forall e. mem e res <==> mem e l /\ e <> ele) /\
-                                 not (member_ele (snd ele) res) /\ not (member_id (fst ele) res) /\
-                                 (forall e. member_id e res <==> member_id e l /\  e <> fst ele) /\
-                                 (forall e. member_ele e res <==> member_ele e l /\ e <> snd ele)))
+                                 not (member_ele_s (snd ele) res) /\ not (member_id_s (fst ele) res) /\
+                                 (forall e. member_id_s e res <==> member_id_s e l /\  e <> fst ele) /\
+                                 (forall e. member_ele_s e res <==> member_ele_s e l /\ e <> snd ele)))
 let rec remove l ele =
   match l with
   |[] -> []
@@ -186,11 +270,11 @@ val diff : a:s
          -> Pure s
              (requires true)
              (ensures (fun d -> (forall e. mem e d <==> mem e a /\ not (mem e l)) /\
-                             (forall e. mem e d /\ member_id (fst e) d <==> 
-                                     mem e a /\ member_id (fst e) a /\ not (mem e l)) /\
-                             (forall e. mem e d  /\ member_ele (snd e) d <==> 
-                                        mem e a /\ member_ele (snd e) a /\ not (mem e l)) /\
-                             (forall e. mem e a /\ mem e l ==> not (member_ele (snd e) d) /\ not (member_id (fst e) d))))
+                             (forall e. mem e d /\ member_id_s (fst e) d <==> 
+                                     mem e a /\ member_id_s (fst e) a /\ not (mem e l)) /\
+                             (forall e. mem e d  /\ member_ele_s (snd e) d <==> 
+                                        mem e a /\ member_ele_s (snd e) a /\ not (mem e l)) /\
+                             (forall e. mem e a /\ mem e l ==> not (member_ele_s (snd e) d) /\ not (member_id_s (fst e) d))))
                              (decreases %[l;a])
 #set-options "--z3rlimit 1000000"
 let rec diff a l = 
@@ -201,7 +285,7 @@ let rec diff a l =
 val get_node : l:s 
              -> ele:nat
              -> Pure (nat * nat)
-                 (requires (member_ele ele l))
+                 (requires (member_ele_s ele l))
                  (ensures (fun e -> mem e l /\ snd e = ele))
 let rec get_node l ele =
   match l with
@@ -210,11 +294,11 @@ let rec get_node l ele =
 val unionst : a:s
             -> b:s
             -> Pure s
-              (requires (forall e. member_id e a ==> not (member_id e b)) /\
-                        (forall e. member_ele e a ==> not (member_ele e b)))
+              (requires (forall e. member_id_s e a ==> not (member_id_s e b)) /\
+                        (forall e. member_ele_s e a ==> not (member_ele_s e b)))
               (ensures (fun r -> (forall e. mem e r <==> mem e a \/ mem e b) /\
-                            (forall e. member_id e r <==> member_id e a \/ member_id e b) /\
-                            (forall e. member_ele e r <==> member_ele e a \/ member_ele e b)))
+                            (forall e. member_id_s e r <==> member_id_s e a \/ member_id_s e b) /\
+                            (forall e. member_ele_s e r <==> member_ele_s e a \/ member_ele_s e b)))
 let rec unionst a b =
   match a,b with
   |[],[] -> []
@@ -223,9 +307,9 @@ let rec unionst a b =
 
 val lemma5 : a:s
            -> b:s
-           -> Lemma (requires (forall e. member_id e a ==> not (member_id e b)))
-                   (ensures (forall e e1. mem e a /\ not (member_ele (snd e) b) /\ 
-                                     mem e1 a /\ member_ele (snd e1) b ==> fst e <> fst e1))
+           -> Lemma (requires (forall e. member_id_s e a ==> not (member_id_s e b)))
+                   (ensures (forall e e1. mem e a /\ not (member_ele_s (snd e) b) /\ 
+                                     mem e1 a /\ member_ele_s (snd e1) b ==> fst e <> fst e1))
 #set-options "--z3rlimit 100000000"
 let rec lemma5 a b = 
   match a, b with
@@ -234,38 +318,38 @@ let rec lemma5 a b =
   |[],_ -> ()
 
 val pre_cond_merge1 : l:s -> a:s -> b:s
-                    -> Tot (b1:bool {b1=true <==> (forall e. member_id e (diff a l) ==> not (member_id e (diff b l))) /\
+                    -> Tot (b1:bool {b1=true <==> (forall e. member_id_s e (diff a l) ==> not (member_id_s e (diff b l))) /\
                         (forall e. (mem e l /\ mem e a /\ mem e b) ==> 
-                              not (member_ele (snd e) (diff a l)) /\ not (member_ele (snd e) (diff b l)) /\
-                              not (member_id (fst e) (diff a l)) /\ not (member_id (fst e) (diff b l))) /\
-                        (forall e. mem e (diff a l) /\ member_ele (snd e) (diff b l) ==> 
+                              not (member_ele_s (snd e) (diff a l)) /\ not (member_ele_s (snd e) (diff b l)) /\
+                              not (member_id_s (fst e) (diff a l)) /\ not (member_id_s (fst e) (diff b l))) /\
+                        (forall e. mem e (diff a l) /\ member_ele_s (snd e) (diff b l) ==> 
                               fst (get_node a (snd e)) <> fst (get_node b (snd e))) /\
-                        (forall e. mem e (diff b l) /\ member_ele (snd e) (diff a l) ==> 
+                        (forall e. mem e (diff b l) /\ member_ele_s (snd e) (diff a l) ==> 
                               fst (get_node b (snd e)) <> fst (get_node a (snd e)))})
 
 #set-options "--z3rlimit 100000000"
 let pre_cond_merge1 l a b =
-  forallb (fun e -> not (member_id (fst e) (diff b l))) (diff a l) &&
-  forallb (fun e -> not (member_ele (snd e) (diff a l)) && not (member_ele (snd e) (diff b l)) &&
-                 not (member_id (fst e) (diff a l)) && not (member_id (fst e) (diff b l))) 
+  forallb (fun e -> not (member_id_s (fst e) (diff b l))) (diff a l) &&
+  forallb (fun e -> not (member_ele_s (snd e) (diff a l)) && not (member_ele_s (snd e) (diff b l)) &&
+                 not (member_id_s (fst e) (diff a l)) && not (member_id_s (fst e) (diff b l))) 
                  (filter (fun e -> mem e a && mem e b) l) &&
-  forallb (fun e -> member_ele (snd e) b && member_ele (snd e) a && fst (get_node b (snd e)) <> fst (get_node a (snd e)))
-                            (filter (fun e -> member_ele (snd e) (diff b l)) (diff a l)) &&
-  forallb (fun e -> member_ele (snd e) b && member_ele (snd e) a && fst (get_node b (snd e)) <> fst (get_node a (snd e)))
-                 (filter (fun e -> member_ele (snd e) (diff a l)) (diff b l))
+  forallb (fun e -> member_ele_s (snd e) b && member_ele_s (snd e) a && fst (get_node b (snd e)) <> fst (get_node a (snd e)))
+                            (filter (fun e -> member_ele_s (snd e) (diff b l)) (diff a l)) &&
+  forallb (fun e -> member_ele_s (snd e) b && member_ele_s (snd e) a && fst (get_node b (snd e)) <> fst (get_node a (snd e)))
+                 (filter (fun e -> member_ele_s (snd e) (diff a l)) (diff b l))
 
 val merge1 : l:s
            -> a:s 
            -> b:s 
            -> Pure s
             (requires pre_cond_merge1 l a b)
-            (ensures (fun res -> (forall e. member_ele e res ==> member_ele e a \/ member_ele e b) /\ 
+            (ensures (fun res -> (forall e. member_ele_s e res ==> member_ele_s e a \/ member_ele_s e b) /\ 
                              (forall e. mem e res <==> (mem e l /\ mem e a /\ mem e b) \/ 
-                         (mem e (diff a l) /\ member_ele (snd e) (diff a l) /\ not (member_ele (snd e) (diff b l))) \/
-                         (mem e (diff b l) /\ member_ele (snd e) (diff b l) /\ not (member_ele (snd e) (diff a l))) \/
-                           (mem e (diff a l) /\ member_ele (snd e) (diff a l) /\ member_ele (snd e) (diff b l) /\
+                         (mem e (diff a l) /\ member_ele_s (snd e) (diff a l) /\ not (member_ele_s (snd e) (diff b l))) \/
+                         (mem e (diff b l) /\ member_ele_s (snd e) (diff b l) /\ not (member_ele_s (snd e) (diff a l))) \/
+                           (mem e (diff a l) /\ member_ele_s (snd e) (diff a l) /\ member_ele_s (snd e) (diff b l) /\
                            fst (get_node a (snd e)) > fst (get_node b (snd e))) \/
-                           (mem e (diff b l) /\ member_ele (snd e) (diff b l) /\ member_ele (snd e) (diff a l) /\
+                           (mem e (diff b l) /\ member_ele_s (snd e) (diff b l) /\ member_ele_s (snd e) (diff a l) /\
                            fst (get_node b (snd e)) > fst (get_node a (snd e))))))
                               (decreases %[(length l); (length a); (length b)])
 
@@ -273,18 +357,18 @@ val merge1 : l:s
 let merge1 l a b = 
   let i = filter (fun e -> mem e a && mem e b) l in
   assert (forall e. mem e i <==> mem e l /\ mem e a /\ mem e b);
-  assert (forall e. member_ele e i ==> member_ele e l /\ member_ele e a /\ member_ele e b);
+  assert (forall e. member_ele_s e i ==> member_ele_s e l /\ member_ele_s e a /\ member_ele_s e b);
   let la = diff a l in let lb = diff b l in
-  let la1 = filter (fun e -> member_ele (snd e) la && not (member_ele (snd e) lb)) la in
-  let lb1 = filter (fun e -> member_ele (snd e) lb && not (member_ele (snd e) la)) lb in
-  let la2 = filter (fun e -> member_ele (snd e) la && member_ele (snd e) lb && 
+  let la1 = filter (fun e -> member_ele_s (snd e) la && not (member_ele_s (snd e) lb)) la in
+  let lb1 = filter (fun e -> member_ele_s (snd e) lb && not (member_ele_s (snd e) la)) lb in
+  let la2 = filter (fun e -> member_ele_s (snd e) la && member_ele_s (snd e) lb && 
                           fst (get_node a (snd e)) > fst (get_node b (snd e))) la in
-  let lb2 = filter (fun e -> member_ele (snd e) la && member_ele (snd e) lb && 
+  let lb2 = filter (fun e -> member_ele_s (snd e) la && member_ele_s (snd e) lb && 
                           fst (get_node b (snd e)) > fst (get_node a (snd e))) lb in
   lemma5 la lb;
-  assert (forall e. member_id e la1 ==> not (member_id e la2));
+  assert (forall e. member_id_s e la1 ==> not (member_id_s e la2));
   lemma5 lb la;
-  assert (forall e. member_id e lb1 ==> not (member_id e lb2));
+  assert (forall e. member_id_s e lb1 ==> not (member_id_s e lb2));
   let u1 = unionst i la1 in
   let u2 = unionst u1 lb1 in
   let u3 = unionst u2 la2 in
@@ -347,7 +431,7 @@ val lemma6 : ltr:ae op
                              (forall e. mem e atr.l ==> not (mem_id (get_id e) btr.l)) /\
                              (forall e. mem e ltr.l ==> not (mem_id (get_id e) btr.l)) /\
                              (sim ltr l /\ sim (union ltr atr) a /\ sim (union ltr btr) b))
-                   (ensures (forall e. member_id e (diff a l) ==> not (member_id e (diff b l))))
+                   (ensures (forall e. member_id_s e (diff a l) ==> not (member_id_s e (diff b l))))
 
 #set-options "--z3rlimit 10000000"
 let lemma6 ltr l atr a btr b = 
@@ -377,7 +461,7 @@ val lemma12 : ltr:ae op
             -> btr:ae op
             -> b:s 
             -> Lemma (requires (pre_cond_merge ltr l atr a btr b))
-                    (ensures (forall e. mem e (diff a l) ==> member_ele (snd e) (merge ltr l atr a btr b)))
+                    (ensures (forall e. mem e (diff a l) ==> member_ele_s (snd e) (merge ltr l atr a btr b)))
 
 #set-options "--z3rlimit 10000000"
 let lemma12 ltr l atr a btr b = 
@@ -390,7 +474,7 @@ val lemma13 : ltr:ae op
             -> btr:ae op
             -> b:s 
             -> Lemma (requires (pre_cond_merge ltr l atr a btr b))
-                    (ensures (forall e. mem e (diff b l) ==> member_ele (snd e) (merge ltr l atr a btr b)))
+                    (ensures (forall e. mem e (diff b l) ==> member_ele_s (snd e) (merge ltr l atr a btr b)))
 
 #set-options "--z3rlimit 10000000"
 let lemma13 ltr l atr a btr b =
@@ -403,7 +487,7 @@ val lemma4 : ltr:ae op
            -> btr:ae op
            -> b:s
            -> Lemma (requires (pre_cond_merge ltr l atr aa btr b) /\
-                             (forall e. member_id e (diff aa l) ==> not (member_id e (diff b l))))
+                             (forall e. member_id_s e (diff aa l) ==> not (member_id_s e (diff b l))))
                    (ensures (forall e. mem e (merge ltr l atr aa btr b) ==>
                             (mem ((fst e), Add (snd e)) (absmerge ltr atr btr).l /\
                     (forall r. mem r (absmerge ltr atr btr).l /\ opr r /\ get_ele r = snd e /\ fst e <> get_id r ==> 
@@ -420,7 +504,7 @@ val lemma31 : ltr:ae op
             -> btr:ae op
             -> b:s
             -> Lemma (requires (pre_cond_merge ltr l atr aa btr b) /\
-                              (forall e. member_id e (diff aa l) ==> not (member_id e (diff b l))))
+                              (forall e. member_id_s e (diff aa l) ==> not (member_id_s e (diff b l))))
                     (ensures (forall e. mem e l /\ mem e aa /\ mem e b ==> 
                              (forall a. mem a (absmerge ltr atr btr).l /\ opa a /\ snd e = get_ele a ==>
              (forall r. mem r (absmerge ltr atr btr).l /\ opr r /\ get_ele a = get_ele r /\ get_id a <> get_id r ==> 
@@ -436,9 +520,9 @@ val lemma32 : ltr:ae op
             -> btr:ae op
             -> b:s
             -> Lemma (requires (pre_cond_merge ltr l atr aa btr b) /\
-                                (forall e. member_id e (diff aa l) ==> not (member_id e (diff b l))))
-                    (ensures (forall e. (mem e (diff aa l) /\ member_ele (snd e) (diff aa l) /\ 
-                                   not (member_ele (snd e) (diff b l))) ==> 
+                                (forall e. member_id_s e (diff aa l) ==> not (member_id_s e (diff b l))))
+                    (ensures (forall e. (mem e (diff aa l) /\ member_ele_s (snd e) (diff aa l) /\ 
+                                   not (member_ele_s (snd e) (diff b l))) ==> 
                                   (forall a. mem a (absmerge ltr atr btr).l /\ opa a /\ snd e = get_ele a ==>
              (forall r. mem r (absmerge ltr atr btr).l /\ opr r /\ get_ele a = get_ele r /\ get_id a <> get_id r ==> 
                                   not ((absmerge ltr atr btr).vis a r)) ==> fst e >= get_id a)))
@@ -460,9 +544,9 @@ val lemma33 : ltr:ae op
             -> btr:ae op
             -> b:s
             -> Lemma (requires (pre_cond_merge ltr l atr aa btr b) /\
-                              (forall e. member_id e (diff aa l) ==> not (member_id e (diff b l))))
-                    (ensures (forall e. (mem e (diff b l) /\ member_ele (snd e) (diff b l) /\ 
-                                not (member_ele (snd e) (diff aa l))) ==> 
+                              (forall e. member_id_s e (diff aa l) ==> not (member_id_s e (diff b l))))
+                    (ensures (forall e. (mem e (diff b l) /\ member_ele_s (snd e) (diff b l) /\ 
+                                not (member_ele_s (snd e) (diff aa l))) ==> 
                                     (forall a. mem a (absmerge ltr atr btr).l /\ opa a /\ snd e = get_ele a ==>
            (forall r. mem r (absmerge ltr atr btr).l /\ opr r /\ get_ele a = get_ele r /\ get_id a <> get_id r ==> 
                                     not ((absmerge ltr atr btr).vis a r)) ==> fst e >= get_id a)))
@@ -484,9 +568,9 @@ val lemma34 : ltr:ae op
             -> btr:ae op
             -> b:s
             -> Lemma (requires (pre_cond_merge ltr l atr aa btr b) /\
-                              (forall e. member_id e (diff aa l) ==> not (member_id e (diff b l))))
-                    (ensures (forall e. (mem e (diff aa l) /\ member_ele (snd e) (diff aa l) /\ 
-                                member_ele (snd e) (diff b l) /\
+                              (forall e. member_id_s e (diff aa l) ==> not (member_id_s e (diff b l))))
+                    (ensures (forall e. (mem e (diff aa l) /\ member_ele_s (snd e) (diff aa l) /\ 
+                                member_ele_s (snd e) (diff b l) /\
                                   fst (get_node aa (snd e)) > fst (get_node b (snd e))) ==> 
                                     (forall a. mem a (absmerge ltr atr btr).l /\ opa a /\ snd e = get_ele a ==>
             (forall r. mem r (absmerge ltr atr btr).l /\ opr r /\ get_ele a = get_ele r /\ get_id a <> get_id r ==> 
@@ -510,8 +594,8 @@ val lemma35 : ltr:ae op
             -> btr:ae op
             -> b:s
             -> Lemma (requires (pre_cond_merge ltr l atr aa btr b) /\
-                              (forall e. member_id e (diff aa l) ==> not (member_id e (diff b l))))
-                    (ensures (forall e. (mem e (diff b l) /\ member_ele (snd e) (diff b l) /\ member_ele (snd e) (diff aa l) /\
+                              (forall e. member_id_s e (diff aa l) ==> not (member_id_s e (diff b l))))
+                    (ensures (forall e. (mem e (diff b l) /\ member_ele_s (snd e) (diff b l) /\ member_ele_s (snd e) (diff aa l) /\
                                   fst (get_node b (snd e)) > fst (get_node aa (snd e))) ==> 
                                     (forall a. mem a (absmerge ltr atr btr).l /\ opa a /\ snd e = get_ele a ==>
            (forall r. mem r (absmerge ltr atr btr).l /\ opr r /\ get_ele a = get_ele r /\ get_id a <> get_id r ==> 
@@ -535,7 +619,7 @@ val lemma3 : ltr:ae op
            -> btr:ae op
            -> b:s
            -> Lemma (requires (pre_cond_merge ltr l atr aa btr b) /\
-                             (forall e. member_id e (diff aa l) ==> not (member_id e (diff b l))))
+                             (forall e. member_id_s e (diff aa l) ==> not (member_id_s e (diff b l))))
                    (ensures (forall e. mem e (merge ltr l atr aa btr b) ==> 
                                 (forall a. mem a (absmerge ltr atr btr).l /\ opa a /\ snd e = get_ele a ==>
        (forall r. mem r (absmerge ltr atr btr).l /\ opr r /\ get_ele a = get_ele r /\ get_id a <> get_id r ==> 
@@ -557,11 +641,11 @@ val lemma21 : ltr:ae op
             -> btr:ae op
             -> b:s 
             -> Lemma (requires (pre_cond_merge ltr l atr aa btr b) /\
-                              (forall e. member_id e (diff aa l) ==> not (member_id e (diff b l))))
+                              (forall e. member_id_s e (diff aa l) ==> not (member_id_s e (diff b l))))
                     (ensures (forall a. mem a ltr.l /\ opa a ==> (forall r. mem r (absmerge ltr atr btr).l /\ 
                                opr r /\ get_ele a = get_ele r /\ get_id a <> get_id r ==> 
                                not ((absmerge ltr atr btr).vis a r)) 
-                                   ==> member_ele (get_ele a) (merge ltr l atr aa btr b)))
+                                   ==> member_ele_s (get_ele a) (merge ltr l atr aa btr b)))
 
 #set-options "--z3rlimit 10000000"
 let lemma21 ltr l atr a btr b = 
@@ -583,11 +667,11 @@ val lemma22 : ltr:ae op
             -> btr:ae op
             -> b:s 
             -> Lemma (requires (pre_cond_merge ltr l atr aa btr b) /\
-                              (forall e. member_id e (diff aa l) ==> not (member_id e (diff b l))))
+                              (forall e. member_id_s e (diff aa l) ==> not (member_id_s e (diff b l))))
                     (ensures (forall a. mem a atr.l /\ opa a ==> (forall r. mem r (absmerge ltr atr btr).l /\ 
                                  opr r /\ get_ele a = get_ele r /\ get_id a <> get_id r ==> 
                                  not ((absmerge ltr atr btr).vis a r)) 
-                                       ==> member_ele (get_ele a) (merge ltr l atr aa btr b)))
+                                       ==> member_ele_s (get_ele a) (merge ltr l atr aa btr b)))
 
 #set-options "--z3rlimit 10000000"
 let lemma22 ltr l atr aa btr b = 
@@ -601,7 +685,7 @@ let lemma22 ltr l atr aa btr b =
   assert (forall e e1. mem e l /\ mem e1 b /\ snd e = snd e1 ==> fst e <= fst e1);
   assert (forall a. mem a atr.l /\ opa a ==> (forall r. mem r (absmerge ltr atr btr).l /\ 
          opr r /\ get_ele a = get_ele r /\ get_id a <> get_id r ==> not ((absmerge ltr atr btr).vis a r))
-                  ==> member_ele (get_ele a) aa);
+                  ==> member_ele_s (get_ele a) aa);
   assert (forall a. mem a atr.l /\ opa a ==> (forall r. mem r (absmerge ltr atr btr).l /\ 
          opr r /\ get_ele a = get_ele r /\ get_id a <> get_id r ==> not ((absmerge ltr atr btr).vis a r)) 
                                      ==> not (mem (get_id a, get_ele a) l)); 
@@ -614,10 +698,10 @@ val lemma23 : ltr:ae op
             -> btr:ae op
             -> b:s 
             -> Lemma (requires (pre_cond_merge ltr l atr aa btr b) /\
-                              (forall e. member_id e (diff aa l) ==> not (member_id e (diff b l))))
+                              (forall e. member_id_s e (diff aa l) ==> not (member_id_s e (diff b l))))
                     (ensures (forall a. mem a btr.l /\ opa a ==> (forall r. mem r (absmerge ltr atr btr).l /\ 
            opr r /\ get_ele a = get_ele r /\ get_id a <> get_id r ==> not ((absmerge ltr atr btr).vis a r)) 
-                                        ==> member_ele (get_ele a) (merge ltr l atr aa btr b)))
+                                        ==> member_ele_s (get_ele a) (merge ltr l atr aa btr b)))
 
 #set-options "--z3rlimit 10000000"
 let lemma23 ltr l atr aa btr b = 
@@ -631,7 +715,7 @@ let lemma23 ltr l atr aa btr b =
   assert (forall e e1. mem e l /\ mem e1 b /\ snd e = snd e1 ==> fst e <= fst e1);
   assert (forall a. mem a btr.l /\ opa a ==> (forall r. mem r (absmerge ltr atr btr).l /\ 
         opr r /\ get_ele a = get_ele r /\ get_id a <> get_id r ==> not ((absmerge ltr atr btr).vis a r)) 
-                               ==> member_ele (get_ele a) b);
+                               ==> member_ele_s (get_ele a) b);
   assert (forall a. mem a btr.l /\ opa a ==> (forall r. mem r (absmerge ltr atr btr).l /\ 
       opr r /\ get_ele a = get_ele r /\ get_id a <> get_id r ==> not ((absmerge ltr atr btr).vis a r)) 
                                ==> not (mem (get_id a, get_ele a) l)); 
@@ -644,11 +728,11 @@ val lemma2 : ltr:ae op
            -> btr:ae op
            -> b:s 
            -> Lemma (requires (pre_cond_merge ltr l atr aa btr b) /\
-                             (forall e. member_id e (diff aa l) ==> not (member_id e (diff b l))))
+                             (forall e. member_id_s e (diff aa l) ==> not (member_id_s e (diff b l))))
                    (ensures (forall a. mem a (absmerge ltr atr btr).l /\ opa a ==> 
                                (forall r. mem r (absmerge ltr atr btr).l /\ 
          opr r /\ get_ele a = get_ele r /\ get_id a <> get_id r ==> not ((absmerge ltr atr btr).vis a r)) 
-                                     ==> member_ele (get_ele a) (merge ltr l atr aa btr b)))
+                                     ==> member_ele_s (get_ele a) (merge ltr l atr aa btr b)))
 
 #set-options "--z3rlimit 10000000"
 let lemma2 ltr l atr a btr b = 
@@ -676,8 +760,20 @@ let prop_merge ltr l atr a btr b =
   lemma4 ltr l atr a btr b;
   ()
 
-instance _ : mrdt s op = {
+val prop_spec : tr:ae op
+                -> st:s
+                -> op:(nat * op)
+                -> Lemma (requires (sim tr st) /\ (not (mem_id (get_id op) tr.l)) /\
+                                   (forall e. mem e tr.l ==> get_id e < get_id op) /\ get_id op > 0)
+                         (ensures (get_op op = Rd ==> (forall e. mem e (extract (get_rval (app_op st op))) <==>
+                                                  mem e (extract (spec op tr)))) /\
+                                  (get_op op <> Rd ==> (get_rval (app_op st op) = spec op tr)))
+#set-options "--z3rlimit 1000000"
+let prop_spec tr st op = ()
+
+instance orset_space : mrdt s op rval = {
   Library.init = init;
+  Library.spec = spec;
   Library.sim = sim;
   Library.pre_cond_op = pre_cond_op;
   Library.app_op = app_op;
@@ -687,6 +783,7 @@ instance _ : mrdt s op = {
   Library.merge1 = merge1;
   Library.merge = merge;
   Library.prop_merge = prop_merge;
+  Library.prop_spec = prop_spec;
   Library.convergence = convergence
 }
 
